src/Forces_Definition.thy
@@ -11,16 +11,16 @@ definition
 
 definition
   frecrelP_fm :: "i \<Rightarrow> i" where
-  "frecrelP_fm(a) == Exists(Exists(And(pair_fm(1,0,a#+2),frecR_fm(1,0))))"
+  "frecrelP_fm(a) \<equiv> Exists(Exists(And(pair_fm(1,0,a#+2),frecR_fm(1,0))))"
 
 lemma arity_frecrelP_fm :
-  "a\<in>nat \<Longrightarrow> arity(frecrelP_fm(a)) =succ(a)" 
+  "a\<in>nat \<Longrightarrow> arity(frecrelP_fm(a)) = succ(a)"
   unfolding frecrelP_fm_def
   using arity_frecR_fm arity_pair_fm pred_Un_distrib
   by simp
 
 lemma frecrelP_fm_type[TC] :
-  "a\<in>nat \<Longrightarrow> frecrelP_fm(a)\<in>formula" 
+  "a\<in>nat \<Longrightarrow> frecrelP_fm(a)\<in>formula"
   unfolding frecrelP_fm_def by simp
 
 lemma sats_frecrelP_fm :
@@ -43,21 +43,21 @@ definition
 
 definition
   frecrel_fm :: "[i,i] \<Rightarrow> i" where
-  "frecrel_fm(a,r) \<equiv> Exists(And(cartprod_fm(a#+1,a#+1,0),Collect_fm(0,frecrelP_fm(0),r#+1)))" 
+  "frecrel_fm(a,r) \<equiv> Exists(And(cartprod_fm(a#+1,a#+1,0),Collect_fm(0,frecrelP_fm(0),r#+1)))"
 
 lemma frecrel_fm_type[TC] :
   "\<lbrakk>a\<in>nat;b\<in>nat\<rbrakk> \<Longrightarrow> frecrel_fm(a,b)\<in>formula"
   unfolding frecrel_fm_def by simp
 
 lemma arity_frecrel_fm :
-  assumes "a\<in>nat"  "b\<in>nat" 
+  assumes "a\<in>nat"  "b\<in>nat"
   shows "arity(frecrel_fm(a,b)) = succ(a) \<union> succ(b)"
   unfolding frecrel_fm_def
-  using assms arity_Collect_fm arity_cartprod_fm arity_frecrelP_fm pred_Un_distrib 
+  using assms arity_Collect_fm arity_cartprod_fm arity_frecrelP_fm pred_Un_distrib
   by auto
 
 lemma sats_frecrel_fm :
-  assumes 
+  assumes
     "a\<in>nat"  "r\<in>nat" "env\<in>list(A)"
   shows
     "sats(A,frecrel_fm(a,r),env)
@@ -87,58 +87,58 @@ lemma names_belowsD:
 
 definition
   is_names_below :: "[i\<Rightarrow>o,i,i,i] \<Rightarrow> o" where
-  "is_names_below(M,P,x,nb) == \<exists>p1[M]. \<exists>p0[M]. \<exists>t[M]. \<exists>ec[M]. 
+  "is_names_below(M,P,x,nb) \<equiv> \<exists>p1[M]. \<exists>p0[M]. \<exists>t[M]. \<exists>ec[M].
               is_ecloseN(M,ec,x) \<and> number2(M,t) \<and> cartprod(M,ec,P,p0) \<and> cartprod(M,ec,p0,p1)
               \<and> cartprod(M,t,p1,nb)"
 
 definition
   number2_fm :: "i\<Rightarrow>i" where
-  "number2_fm(a) == Exists(And(number1_fm(0), succ_fm(0,succ(a))))"
+  "number2_fm(a) \<equiv> Exists(And(number1_fm(0), succ_fm(0,succ(a))))"
 
 lemma number2_fm_type[TC] :
   "a\<in>nat \<Longrightarrow> number2_fm(a) \<in> formula"
   unfolding number2_fm_def by simp
 
-lemma number2arity__fm : 
+lemma number2arity__fm :
   "a\<in>nat \<Longrightarrow> arity(number2_fm(a)) = succ(a)"
   unfolding number2_fm_def
   using number1arity__fm arity_succ_fm nat_union_abs2 pred_Un_distrib
   by simp
 
 lemma sats_number2_fm [simp]:
-  "[| x \<in> nat; env \<in> list(A)|]
-    ==> sats(A, number2_fm(x), env) \<longleftrightarrow> number2(##A, nth(x,env))"
+  "\<lbrakk> x \<in> nat; env \<in> list(A) \<rbrakk>
+    \<Longrightarrow> sats(A, number2_fm(x), env) \<longleftrightarrow> number2(##A, nth(x,env))"
   by (simp add: number2_fm_def number2_def)
 
-definition 
+definition
   is_names_below_fm :: "[i,i,i] \<Rightarrow> i" where
-  "is_names_below_fm(P,x,nb) == Exists(Exists(Exists(Exists(
+  "is_names_below_fm(P,x,nb) \<equiv> Exists(Exists(Exists(Exists(
                     And(ecloseN_fm(0,x #+ 4),And(number2_fm(1),
                     And(cartprod_fm(0,P #+ 4,2),And(cartprod_fm(0,2,3),cartprod_fm(1,3,nb#+4)))))))))"
 
-lemma arity_is_names_below_fm : 
+lemma arity_is_names_below_fm :
   "\<lbrakk>P\<in>nat;x\<in>nat;nb\<in>nat\<rbrakk> \<Longrightarrow> arity(is_names_below_fm(P,x,nb)) = succ(P) \<union> succ(x) \<union> succ(nb)"
-  unfolding is_names_below_fm_def 
+  unfolding is_names_below_fm_def
   using arity_cartprod_fm number2arity__fm arity_ecloseN_fm nat_union_abs2 pred_Un_distrib
   by auto
 
 
 lemma is_names_below_fm_type[TC]:
-  "\<lbrakk>P\<in>nat;x\<in>nat;nb\<in>nat\<rbrakk> \<Longrightarrow> is_names_below_fm(P,x,nb)\<in>formula" 
+  "\<lbrakk>P\<in>nat;x\<in>nat;nb\<in>nat\<rbrakk> \<Longrightarrow> is_names_below_fm(P,x,nb)\<in>formula"
   unfolding is_names_below_fm_def by simp
 
 lemma sats_is_names_below_fm :
   assumes
-    "P\<in>nat" "x\<in>nat" "nb\<in>nat" "env\<in>list(A)" 
+    "P\<in>nat" "x\<in>nat" "nb\<in>nat" "env\<in>list(A)"
   shows
     "sats(A,is_names_below_fm(P,x,nb),env)
-    \<longleftrightarrow> is_names_below(##A,nth(P, env),nth(x, env),nth(nb, env))" 
+    \<longleftrightarrow> is_names_below(##A,nth(P, env),nth(x, env),nth(nb, env))"
   unfolding is_names_below_fm_def is_names_below_def using assms by simp
 
 definition
   is_tuple :: "[i\<Rightarrow>o,i,i,i,i,i] \<Rightarrow> o" where
-  "is_tuple(M,z,t1,t2,p,t) == \<exists>t1t2p[M]. \<exists>t2p[M]. pair(M,t2,p,t2p) \<and> pair(M,t1,t2p,t1t2p) \<and>
-                                                  pair(M,z,t1t2p,t)" 
+  "is_tuple(M,z,t1,t2,p,t) \<equiv> \<exists>t1t2p[M]. \<exists>t2p[M]. pair(M,t2,p,t2p) \<and> pair(M,t1,t2p,t1t2p) \<and>
+                                                  pair(M,z,t1t2p,t)"
 
 
 definition
@@ -147,14 +147,14 @@ definition
                       And(pair_fm(t1 #+ 2,0,1),pair_fm(z #+ 2,1,tup #+ 2)))))"
 
 
-lemma arity_is_tuple_fm : "\<lbrakk> z\<in>nat ; t1\<in>nat ; t2\<in>nat ; p\<in>nat ; tup\<in>nat \<rbrakk> \<Longrightarrow> 
+lemma arity_is_tuple_fm : "\<lbrakk> z\<in>nat ; t1\<in>nat ; t2\<in>nat ; p\<in>nat ; tup\<in>nat \<rbrakk> \<Longrightarrow>
   arity(is_tuple_fm(z,t1,t2,p,tup)) = \<Union> {succ(z),succ(t1),succ(t2),succ(p),succ(tup)}"
   unfolding is_tuple_fm_def
   using arity_pair_fm nat_union_abs1 nat_union_abs2 pred_Un_distrib
   by auto
 
-lemma is_tuple_fm_type[TC] : 
-  "z\<in>nat \<Longrightarrow> t1\<in>nat \<Longrightarrow> t2\<in>nat \<Longrightarrow> p\<in>nat \<Longrightarrow> tup\<in>nat \<Longrightarrow> is_tuple_fm(z,t1,t2,p,tup)\<in>formula" 
+lemma is_tuple_fm_type[TC] :
+  "z\<in>nat \<Longrightarrow> t1\<in>nat \<Longrightarrow> t2\<in>nat \<Longrightarrow> p\<in>nat \<Longrightarrow> tup\<in>nat \<Longrightarrow> is_tuple_fm(z,t1,t2,p,tup)\<in>formula"
   unfolding is_tuple_fm_def by simp
 
 lemma sats_is_tuple_fm :
@@ -190,7 +190,7 @@ definition
        \<longrightarrow> (\<forall>q[M]. q\<in>P \<and> (\<exists>qp[M]. pair(M,q,p,qp) \<and> qp\<in>leq) \<longrightarrow>
             (\<exists>ost1q[M]. \<exists>ost2q[M]. \<exists>o[M].  \<exists>vf1[M]. \<exists>vf2[M].
              is_tuple(M,o,s,t1,q,ost1q) \<and>
-             is_tuple(M,o,s,t2,q,ost2q) \<and> number1(M,o) \<and> 
+             is_tuple(M,o,s,t2,q,ost2q) \<and> number1(M,o) \<and>
              fun_apply(M,f,ost1q,vf1) \<and> fun_apply(M,f,ost2q,vf2) \<and>
              (vf1 = o \<longleftrightarrow> vf2 = o)))"
 
@@ -205,28 +205,28 @@ definition
   is_mem_case :: "[i\<Rightarrow>o,i,i,i,i,i,i] \<Rightarrow> o" where
   "is_mem_case(M,t1,t2,p,P,leq,f) \<equiv> \<forall>v[M]. \<forall>vp[M]. v\<in>P \<and> pair(M,v,p,vp) \<and> vp\<in>leq \<longrightarrow>
     (\<exists>q[M]. \<exists>s[M]. \<exists>r[M]. \<exists>qv[M]. \<exists>sr[M]. \<exists>qr[M]. \<exists>z[M]. \<exists>zt1sq[M]. \<exists>o[M].
-     r\<in> P \<and> q\<in>P \<and> pair(M,q,v,qv) \<and> pair(M,s,r,sr) \<and> pair(M,q,r,qr) \<and> 
+     r\<in> P \<and> q\<in>P \<and> pair(M,q,v,qv) \<and> pair(M,s,r,sr) \<and> pair(M,q,r,qr) \<and>
      empty(M,z) \<and> is_tuple(M,z,t1,s,q,zt1sq) \<and>
      number1(M,o) \<and> qv\<in>leq \<and> sr\<in>t2 \<and> qr\<in>leq \<and> fun_apply(M,f,zt1sq,o))"
 
 
 schematic_goal sats_is_mem_case_fm_auto:
-  assumes 
+  assumes
     "n1\<in>nat" "n2\<in>nat" "p\<in>nat" "P\<in>nat" "leq\<in>nat" "f\<in>nat" "env\<in>list(A)"
   shows
     "is_mem_case(##A, nth(n1, env),nth(n2, env),nth(p, env),nth(P, env), nth(leq, env),nth(f,env))
     \<longleftrightarrow> sats(A,?imc_fm(n1,n2,p,P,leq,f),env)"
-  unfolding is_mem_case_def 
+  unfolding is_mem_case_def
   by (insert assms ; (rule sep_rules'  is_tuple_iff_sats | simp)+)
 
 
 synthesize "mem_case_fm" from_schematic "sats_is_mem_case_fm_auto"
 
-lemma arity_mem_case_fm : 
-  assumes 
+lemma arity_mem_case_fm :
+  assumes
     "n1\<in>nat" "n2\<in>nat" "p\<in>nat" "P\<in>nat" "leq\<in>nat" "f\<in>nat"
   shows
-    "arity(mem_case_fm(n1,n2,p,P,leq,f)) = 
+    "arity(mem_case_fm(n1,n2,p,P,leq,f)) =
     succ(n1) \<union> succ(n2) \<union> succ(p) \<union> succ(P) \<union> succ(leq) \<union> succ(f)"
   unfolding mem_case_fm_def
   using assms arity_pair_fm arity_is_tuple_fm number1arity__fm arity_fun_apply_fm arity_empty_fm
@@ -234,7 +234,7 @@ lemma arity_mem_case_fm :
   by auto
 
 schematic_goal sats_is_eq_case_fm_auto:
-  assumes 
+  assumes
     "n1\<in>nat" "n2\<in>nat" "p\<in>nat" "P\<in>nat" "leq\<in>nat" "f\<in>nat" "env\<in>list(A)"
   shows
     "is_eq_case(##A, nth(n1, env),nth(n2, env),nth(p, env),nth(P, env), nth(leq, env),nth(f,env))
@@ -244,11 +244,11 @@ schematic_goal sats_is_eq_case_fm_auto:
 
 synthesize "eq_case_fm" from_schematic "sats_is_eq_case_fm_auto"
 
-lemma arity_eq_case_fm : 
-  assumes 
+lemma arity_eq_case_fm :
+  assumes
     "n1\<in>nat" "n2\<in>nat" "p\<in>nat" "P\<in>nat" "leq\<in>nat" "f\<in>nat"
   shows
-    "arity(eq_case_fm(n1,n2,p,P,leq,f)) = 
+    "arity(eq_case_fm(n1,n2,p,P,leq,f)) =
     succ(n1) \<union> succ(n2) \<union> succ(p) \<union> succ(P) \<union> succ(leq) \<union> succ(f)"
   unfolding eq_case_fm_def
   using assms arity_pair_fm arity_is_tuple_fm number1arity__fm arity_fun_apply_fm arity_empty_fm
@@ -264,26 +264,26 @@ lemma eq_case_fm_type[TC] :
   unfolding eq_case_fm_def by simp
 
 lemma sats_eq_case_fm :
-  assumes 
+  assumes
     "n1\<in>nat" "n2\<in>nat" "p\<in>nat" "P\<in>nat" "leq\<in>nat" "f\<in>nat" "env\<in>list(A)"
   shows
-    "sats(A,eq_case_fm(n1,n2,p,P,leq,f),env) \<longleftrightarrow> 
+    "sats(A,eq_case_fm(n1,n2,p,P,leq,f),env) \<longleftrightarrow>
     is_eq_case(##A, nth(n1, env),nth(n2, env),nth(p, env),nth(P, env), nth(leq, env),nth(f,env))"
   unfolding eq_case_fm_def is_eq_case_def using assms by (simp add: sats_is_tuple_fm)
 
 lemma sats_mem_case_fm :
-  assumes 
+  assumes
     "n1\<in>nat" "n2\<in>nat" "p\<in>nat" "P\<in>nat" "leq\<in>nat" "f\<in>nat" "env\<in>list(A)"
   shows
-    "sats(A,mem_case_fm(n1,n2,p,P,leq,f),env) \<longleftrightarrow> 
+    "sats(A,mem_case_fm(n1,n2,p,P,leq,f),env) \<longleftrightarrow>
     is_mem_case(##A, nth(n1, env),nth(n2, env),nth(p, env),nth(P, env), nth(leq, env),nth(f,env))"
   unfolding mem_case_fm_def is_mem_case_def using assms by (simp add: sats_is_tuple_fm)
 
 lemma mem_case_iff_sats:
   assumes
-    "n1\<in>nat" "n2\<in>nat" "p\<in>nat" "P\<in>nat" "leq\<in>nat" "f\<in>nat" "env\<in>list(A)"    
-    "nth(n1,env) = nn1" "nth(n2,env) = nn2" "nth(p,env) = pp" "nth(P,env) = PP" 
-    "nth(leq,env) = lleq" "nth(f,env) = ff"  
+    "n1\<in>nat" "n2\<in>nat" "p\<in>nat" "P\<in>nat" "leq\<in>nat" "f\<in>nat" "env\<in>list(A)"
+    "nth(n1,env) = nn1" "nth(n2,env) = nn2" "nth(p,env) = pp" "nth(P,env) = PP"
+    "nth(leq,env) = lleq" "nth(f,env) = ff"
   shows
     "is_mem_case(##A, nn1,nn2,pp,PP, lleq,ff)
     \<longleftrightarrow> sats(A,mem_case_fm(n1,n2,p,P,leq,f),env)"
@@ -292,9 +292,9 @@ lemma mem_case_iff_sats:
 
 lemma eq_case_iff_sats :
   assumes
-    "n1\<in>nat" "n2\<in>nat" "p\<in>nat" "P\<in>nat" "leq\<in>nat" "f\<in>nat" "env\<in>list(A)"    
-    "nth(n1,env) = nn1" "nth(n2,env) = nn2" "nth(p,env) = pp" "nth(P,env) = PP" 
-    "nth(leq,env) = lleq" "nth(f,env) = ff"  
+    "n1\<in>nat" "n2\<in>nat" "p\<in>nat" "P\<in>nat" "leq\<in>nat" "f\<in>nat" "env\<in>list(A)"
+    "nth(n1,env) = nn1" "nth(n2,env) = nn2" "nth(p,env) = pp" "nth(P,env) = PP"
+    "nth(leq,env) = lleq" "nth(f,env) = ff"
   shows
     "is_eq_case(##A, nn1,nn2,pp,PP, lleq,ff)
     \<longleftrightarrow> sats(A,eq_case_fm(n1,n2,p,P,leq,f),env)"
@@ -310,14 +310,14 @@ definition
 definition
   is_Hfrc :: "[i\<Rightarrow>o,i,i,i,i] \<Rightarrow> o" where
   "is_Hfrc(M,P,leq,fnnc,f) \<equiv>
-     \<exists>ft[M]. \<exists>n1[M]. \<exists>n2[M]. \<exists>co[M]. 
+     \<exists>ft[M]. \<exists>n1[M]. \<exists>n2[M]. \<exists>co[M].
       co\<in>P \<and> is_tuple(M,ft,n1,n2,co,fnnc) \<and>
       (  (empty(M,ft) \<and> is_eq_case(M,n1,n2,co,P,leq,f))
        \<or> (number1(M,ft) \<and>  is_mem_case(M,n1,n2,co,P,leq,f)))"
 
-definition 
+definition
   Hfrc_fm :: "[i,i,i,i] \<Rightarrow> i" where
-  "Hfrc_fm(P,leq,fnnc,f) \<equiv> 
+  "Hfrc_fm(P,leq,fnnc,f) \<equiv>
     Exists(Exists(Exists(Exists(
       And(Member(0,P #+ 4),And(is_tuple_fm(3,2,1,0,fnnc #+ 4),
       Or(And(empty_fm(3),eq_case_fm(2,1,0,P #+ 4,leq #+ 4,f #+ 4)),
@@ -327,8 +327,8 @@ lemma Hfrc_fm_type[TC] :
   "\<lbrakk>P\<in>nat;leq\<in>nat;fnnc\<in>nat;f\<in>nat\<rbrakk> \<Longrightarrow> Hfrc_fm(P,leq,fnnc,f)\<in>formula"
   unfolding Hfrc_fm_def by simp
 
-lemma arity_Hfrc_fm : 
-  assumes 
+lemma arity_Hfrc_fm :
+  assumes
     "P\<in>nat" "leq\<in>nat" "fnnc\<in>nat" "f\<in>nat"
   shows
     "arity(Hfrc_fm(P,leq,fnnc,f)) = succ(P) \<union> succ(leq) \<union> succ(fnnc) \<union> succ(f)"
@@ -338,19 +338,19 @@ lemma arity_Hfrc_fm :
   by auto
 
 lemma sats_Hfrc_fm:
-  assumes 
+  assumes
     "P\<in>nat" "leq\<in>nat" "fnnc\<in>nat" "f\<in>nat" "env\<in>list(A)"
   shows
     "sats(A,Hfrc_fm(P,leq,fnnc,f),env)
     \<longleftrightarrow> is_Hfrc(##A,nth(P, env), nth(leq, env), nth(fnnc, env),nth(f, env))"
-  unfolding is_Hfrc_def Hfrc_fm_def 
+  unfolding is_Hfrc_def Hfrc_fm_def
   using assms
   by (simp add:sats_eq_case_fm sats_is_tuple_fm sats_mem_case_fm)
 
 lemma Hfrc_iff_sats:
   assumes
-    "P\<in>nat" "leq\<in>nat" "fnnc\<in>nat" "f\<in>nat" "env\<in>list(A)"    
-    "nth(P,env) = PP"  "nth(leq,env) = lleq" "nth(fnnc,env) = ffnnc" "nth(f,env) = ff" 
+    "P\<in>nat" "leq\<in>nat" "fnnc\<in>nat" "f\<in>nat" "env\<in>list(A)"
+    "nth(P,env) = PP"  "nth(leq,env) = lleq" "nth(fnnc,env) = ffnnc" "nth(f,env) = ff"
   shows
     "is_Hfrc(##A, PP, lleq,ffnnc,ff)
     \<longleftrightarrow> sats(A,Hfrc_fm(P,leq,fnnc,f),env)"
@@ -359,17 +359,17 @@ lemma Hfrc_iff_sats:
 
 definition
   is_Hfrc_at :: "[i\<Rightarrow>o,i,i,i,i,i] \<Rightarrow> o" where
-  "is_Hfrc_at(M,P,leq,fnnc,f,z) \<equiv> 
+  "is_Hfrc_at(M,P,leq,fnnc,f,z) \<equiv>
             (empty(M,z) \<and> \<not> is_Hfrc(M,P,leq,fnnc,f))
           \<or> (number1(M,z) \<and> is_Hfrc(M,P,leq,fnnc,f))"
 
 definition
   Hfrc_at_fm :: "[i,i,i,i,i] \<Rightarrow> i" where
   "Hfrc_at_fm(P,leq,fnnc,f,z) \<equiv> Or(And(empty_fm(z),Neg(Hfrc_fm(P,leq,fnnc,f))),
-                                      And(number1_fm(z),Hfrc_fm(P,leq,fnnc,f)))" 
+                                      And(number1_fm(z),Hfrc_fm(P,leq,fnnc,f)))"
 
 lemma arity_Hfrc_at_fm :
-  assumes 
+  assumes
     "P\<in>nat" "leq\<in>nat" "fnnc\<in>nat" "f\<in>nat" "z\<in>nat"
   shows
     "arity(Hfrc_at_fm(P,leq,fnnc,f,z)) = succ(P) \<union> succ(leq) \<union> succ(fnnc) \<union> succ(f) \<union> succ(z)"
@@ -383,7 +383,7 @@ lemma Hfrc_at_fm_type[TC] :
   unfolding Hfrc_at_fm_def by simp
 
 lemma sats_Hfrc_at_fm:
-  assumes 
+  assumes
     "P\<in>nat" "leq\<in>nat" "fnnc\<in>nat" "f\<in>nat" "z\<in>nat" "env\<in>list(A)"
   shows
     "sats(A,Hfrc_at_fm(P,leq,fnnc,f,z),env)
@@ -393,8 +393,8 @@ lemma sats_Hfrc_at_fm:
 
 lemma is_Hfrc_at_iff_sats:
   assumes
-    "P\<in>nat" "leq\<in>nat" "fnnc\<in>nat" "f\<in>nat" "z\<in>nat" "env\<in>list(A)"    
-    "nth(P,env) = PP"  "nth(leq,env) = lleq" "nth(fnnc,env) = ffnnc" 
+    "P\<in>nat" "leq\<in>nat" "fnnc\<in>nat" "f\<in>nat" "z\<in>nat" "env\<in>list(A)"
+    "nth(P,env) = PP"  "nth(leq,env) = lleq" "nth(fnnc,env) = ffnnc"
     "nth(f,env) = ff" "nth(z,env) = zz"
   shows
     "is_Hfrc_at(##A, PP, lleq,ffnnc,ff,zz)
@@ -404,7 +404,7 @@ lemma is_Hfrc_at_iff_sats:
 
 lemma arity_tran_closure_fm :
   "\<lbrakk>x\<in>nat;f\<in>nat\<rbrakk> \<Longrightarrow> arity(tran_closure_fm(x,f)) = succ(x) \<union> succ(f)"
-  unfolding tran_closure_fm_def 
+  unfolding tran_closure_fm_def
   using arity_omega_fm arity_field_fm arity_typed_function_fm arity_pair_fm arity_empty_fm arity_fun_apply_fm
     arity_composition_fm arity_succ_fm nat_union_abs2 pred_Un_distrib
   by auto
@@ -416,28 +416,28 @@ definition
 
 definition
   is_forcerel :: "[i\<Rightarrow>o,i,i,i] \<Rightarrow> o" where
-  "is_forcerel(M,P,x,z) == \<exists>r[M]. \<exists>nb[M]. tran_closure(M,r,z) \<and> 
+  "is_forcerel(M,P,x,z) \<equiv> \<exists>r[M]. \<exists>nb[M]. tran_closure(M,r,z) \<and>
                         (is_names_below(M,P,x,nb) \<and> is_frecrel(M,nb,r))"
 
 definition
   forcerel_fm :: "i\<Rightarrow> i \<Rightarrow> i \<Rightarrow> i" where
-  "forcerel_fm(p,x,z) == Exists(Exists(And(tran_closure_fm(1, z#+2),
+  "forcerel_fm(p,x,z) \<equiv> Exists(Exists(And(tran_closure_fm(1, z#+2),
                                         And(is_names_below_fm(p#+2,x#+2,0),frecrel_fm(0,1)))))"
 
-lemma arity_forcerel_fm: 
-  "\<lbrakk>p\<in>nat;x\<in>nat;z\<in>nat\<rbrakk> \<Longrightarrow> arity(forcerel_fm(p,x,z)) = succ(p) \<union> succ(x) \<union> succ(z)" 
-  unfolding forcerel_fm_def 
+lemma arity_forcerel_fm:
+  "\<lbrakk>p\<in>nat;x\<in>nat;z\<in>nat\<rbrakk> \<Longrightarrow> arity(forcerel_fm(p,x,z)) = succ(p) \<union> succ(x) \<union> succ(z)"
+  unfolding forcerel_fm_def
   using arity_frecrel_fm arity_tran_closure_fm arity_is_names_below_fm pred_Un_distrib
   by auto
 
-lemma forcerel_fm_type[TC]: 
-  "\<lbrakk>p\<in>nat;x\<in>nat;z\<in>nat\<rbrakk> \<Longrightarrow> forcerel_fm(p,x,z)\<in>formula" 
+lemma forcerel_fm_type[TC]:
+  "\<lbrakk>p\<in>nat;x\<in>nat;z\<in>nat\<rbrakk> \<Longrightarrow> forcerel_fm(p,x,z)\<in>formula"
   unfolding forcerel_fm_def by simp
 
 
 lemma sats_forcerel_fm:
   assumes
-    "p\<in>nat" "x\<in>nat"  "z\<in>nat" "env\<in>list(A)" 
+    "p\<in>nat" "x\<in>nat"  "z\<in>nat" "env\<in>list(A)"
   shows
     "sats(A,forcerel_fm(p,x,z),env) \<longleftrightarrow> is_forcerel(##A,nth(p,env),nth(x, env),nth(z, env))"
 proof -
@@ -450,7 +450,7 @@ proof -
     if "r\<in>A" "nb\<in>A" for nb r
     using assms that sats_is_names_below_fm[of "p #+ 2" "x #+ 2" 0 "[nb,r]@env"] by simp
   moreover
-  have "sats(A, frecrel_fm(0, 1), Cons(nb, Cons(r, env))) \<longleftrightarrow> 
+  have "sats(A, frecrel_fm(0, 1), Cons(nb, Cons(r, env))) \<longleftrightarrow>
         is_frecrel(##A, nb, r)"
     if "r\<in>A" "nb\<in>A" for r nb
     using assms that sats_frecrel_fm[of 0 1 "[nb,r]@env"] by simp
@@ -466,12 +466,12 @@ definition
 
 definition
   is_frc_at :: "[i\<Rightarrow>o,i,i,i,i] \<Rightarrow> o" where
-  "is_frc_at(M,P,leq,x,z) \<equiv> \<exists>r[M]. is_forcerel(M,P,x,r) \<and> 
+  "is_frc_at(M,P,leq,x,z) \<equiv> \<exists>r[M]. is_forcerel(M,P,x,r) \<and>
                                     is_wfrec(M,is_Hfrc_at(M,P,leq),r,x,z)"
 
 definition
   frc_at_fm :: "[i,i,i,i] \<Rightarrow> i" where
-  "frc_at_fm(p,l,x,z) == Exists(And(forcerel_fm(succ(p),succ(x),0),
+  "frc_at_fm(p,l,x,z) \<equiv> Exists(And(forcerel_fm(succ(p),succ(x),0),
           is_wfrec_fm(Hfrc_at_fm(6#+p,6#+l,2,1,0),0,succ(x),succ(z))))"
 
 lemma frc_at_fm_type [TC] :
@@ -480,14 +480,14 @@ lemma frc_at_fm_type [TC] :
 
 lemma arity_frc_at_fm :
   assumes "p\<in>nat" "l\<in>nat" "x\<in>nat" "z\<in>nat"
-  shows "arity(frc_at_fm(p,l,x,z)) = succ(p) \<union> succ(l) \<union> succ(x) \<union> succ(z)" 
+  shows "arity(frc_at_fm(p,l,x,z)) = succ(p) \<union> succ(l) \<union> succ(x) \<union> succ(z)"
 proof -
   let ?\<phi> = "Hfrc_at_fm(6 #+ p, 6 #+ l, 2, 1, 0)"
   from assms
   have  "arity(?\<phi>) = (7#+p) \<union> (7#+l)" "?\<phi> \<in> formula"
     using arity_Hfrc_at_fm nat_simp_union
     by auto
-  with assms 
+  with assms
   have W: "arity(is_wfrec_fm(?\<phi>, 0, succ(x), succ(z))) = 2#+p \<union> (2#+l) \<union> (2#+x) \<union> (2#+z)"
     using arity_is_wfrec_fm[OF \<open>?\<phi>\<in>_\<close> _ _ _ _ \<open>arity(?\<phi>) = _\<close>] pred_Un_distrib pred_succ_eq
       nat_union_abs1
@@ -497,8 +497,8 @@ proof -
     using arity_forcerel_fm nat_simp_union
     by auto
   with W assms
-  show ?thesis 
-    unfolding frc_at_fm_def 
+  show ?thesis
+    unfolding frc_at_fm_def
     using arity_forcerel_fm pred_Un_distrib
     by auto
 qed
@@ -507,21 +507,21 @@ lemma sats_frc_at_fm :
   assumes
     "p\<in>nat" "l\<in>nat" "i\<in>nat" "j\<in>nat" "env\<in>list(A)" "i < length(env)" "j < length(env)"
   shows
-    "sats(A,frc_at_fm(p,l,i,j),env) \<longleftrightarrow> 
-     is_frc_at(##A,nth(p,env),nth(l,env),nth(i,env),nth(j,env))" 
+    "sats(A,frc_at_fm(p,l,i,j),env) \<longleftrightarrow>
+     is_frc_at(##A,nth(p,env),nth(l,env),nth(i,env),nth(j,env))"
 proof -
   {
     fix r pp ll
-    assume "r\<in>A" 
-    have 0:"is_Hfrc_at(##A,nth(p,env),nth(l,env),a2, a1, a0) \<longleftrightarrow> 
-         sats(A, Hfrc_at_fm(6#+p,6#+l,2,1,0), [a0,a1,a2,a3,a4,r]@env)" 
+    assume "r\<in>A"
+    have 0:"is_Hfrc_at(##A,nth(p,env),nth(l,env),a2, a1, a0) \<longleftrightarrow>
+         sats(A, Hfrc_at_fm(6#+p,6#+l,2,1,0), [a0,a1,a2,a3,a4,r]@env)"
       if "a0\<in>A" "a1\<in>A" "a2\<in>A" "a3\<in>A" "a4\<in>A" for a0 a1 a2 a3 a4
-      using  that assms \<open>r\<in>A\<close> 
+      using  that assms \<open>r\<in>A\<close>
         is_Hfrc_at_iff_sats[of "6#+p" "6#+l" 2 1 0 "[a0,a1,a2,a3,a4,r]@env" A]  by simp
     have "sats(A,is_wfrec_fm(Hfrc_at_fm(6 #+ p, 6 #+ l, 2, 1, 0), 0, succ(i), succ(j)),[r]@env) \<longleftrightarrow>
          is_wfrec(##A, is_Hfrc_at(##A, nth(p,env), nth(l,env)), r,nth(i, env), nth(j, env))"
-      using assms \<open>r\<in>A\<close> 
-        sats_is_wfrec_fm[OF 0[simplified]]  
+      using assms \<open>r\<in>A\<close>
+        sats_is_wfrec_fm[OF 0[simplified]]
       by simp
   }
   moreover
@@ -551,12 +551,12 @@ definition
 
 definition
   is_forces_eq' :: "[i\<Rightarrow>o,i,i,i,i,i] \<Rightarrow> o" where
-  "is_forces_eq'(M,P,l,p,t1,t2) == \<exists>o[M]. \<exists>z[M]. \<exists>t[M]. number1(M,o) \<and> empty(M,z) \<and> 
+  "is_forces_eq'(M,P,l,p,t1,t2) \<equiv> \<exists>o[M]. \<exists>z[M]. \<exists>t[M]. number1(M,o) \<and> empty(M,z) \<and>
                                 is_tuple(M,z,t1,t2,p,t) \<and> is_frc_at(M,P,l,t,o)"
 
 definition
   is_forces_mem' :: "[i\<Rightarrow>o,i,i,i,i,i] \<Rightarrow> o" where
-  "is_forces_mem'(M,P,l,p,t1,t2) == \<exists>o[M]. \<exists>t[M]. number1(M,o) \<and>  
+  "is_forces_mem'(M,P,l,p,t1,t2) \<equiv> \<exists>o[M]. \<exists>t[M]. number1(M,o) \<and>
                                 is_tuple(M,o,t1,t2,p,t) \<and> is_frc_at(M,P,l,t,o)"
 
 definition
@@ -571,7 +571,7 @@ definition
 
 definition
   forces_eq_fm :: "[i,i,i,i,i] \<Rightarrow> i" where
-  "forces_eq_fm(p,l,q,t1,t2) \<equiv> 
+  "forces_eq_fm(p,l,q,t1,t2) \<equiv>
      Exists(Exists(Exists(And(number1_fm(2),And(empty_fm(1),
               And(is_tuple_fm(1,t1#+3,t2#+3,q#+3,0),frc_at_fm(p#+3,l#+3,0,2) ))))))"
 
@@ -593,7 +593,7 @@ definition
 
 lemma forces_eq_fm_type [TC]:
   "\<lbrakk> p\<in>nat;l\<in>nat;q\<in>nat;t1\<in>nat;t2\<in>nat\<rbrakk> \<Longrightarrow> forces_eq_fm(p,l,q,t1,t2) \<in> formula"
-  unfolding forces_eq_fm_def 
+  unfolding forces_eq_fm_def
   by simp
 
 lemma forces_mem_fm_type [TC]:
@@ -603,57 +603,57 @@ lemma forces_mem_fm_type [TC]:
 
 lemma forces_neq_fm_type [TC]:
   "\<lbrakk> p\<in>nat;l\<in>nat;q\<in>nat;t1\<in>nat;t2\<in>nat\<rbrakk> \<Longrightarrow> forces_neq_fm(p,l,q,t1,t2) \<in> formula"
-  unfolding forces_neq_fm_def 
+  unfolding forces_neq_fm_def
   by simp
 
 lemma forces_nmem_fm_type [TC]:
   "\<lbrakk> p\<in>nat;l\<in>nat;q\<in>nat;t1\<in>nat;t2\<in>nat\<rbrakk> \<Longrightarrow> forces_nmem_fm(p,l,q,t1,t2) \<in> formula"
-  unfolding forces_nmem_fm_def 
+  unfolding forces_nmem_fm_def
   by simp
 
 lemma arity_forces_eq_fm :
-  "p\<in>nat \<Longrightarrow> l\<in>nat \<Longrightarrow> q\<in>nat \<Longrightarrow> t1 \<in> nat \<Longrightarrow> t2 \<in> nat \<Longrightarrow> 
+  "p\<in>nat \<Longrightarrow> l\<in>nat \<Longrightarrow> q\<in>nat \<Longrightarrow> t1 \<in> nat \<Longrightarrow> t2 \<in> nat \<Longrightarrow>
    arity(forces_eq_fm(p,l,q,t1,t2)) = succ(t1) \<union> succ(t2) \<union> succ(q) \<union> succ(p) \<union> succ(l)"
-  unfolding forces_eq_fm_def 
+  unfolding forces_eq_fm_def
   using number1arity__fm arity_empty_fm arity_is_tuple_fm arity_frc_at_fm
     pred_Un_distrib
   by auto
 
 lemma arity_forces_mem_fm :
-  "p\<in>nat \<Longrightarrow> l\<in>nat \<Longrightarrow> q\<in>nat \<Longrightarrow> t1 \<in> nat \<Longrightarrow> t2 \<in> nat \<Longrightarrow> 
+  "p\<in>nat \<Longrightarrow> l\<in>nat \<Longrightarrow> q\<in>nat \<Longrightarrow> t1 \<in> nat \<Longrightarrow> t2 \<in> nat \<Longrightarrow>
    arity(forces_mem_fm(p,l,q,t1,t2)) = succ(t1) \<union> succ(t2) \<union> succ(q) \<union> succ(p) \<union> succ(l)"
-  unfolding forces_mem_fm_def 
+  unfolding forces_mem_fm_def
   using number1arity__fm arity_empty_fm arity_is_tuple_fm arity_frc_at_fm
     pred_Un_distrib
   by auto
 
-lemma sats_forces_eq'_fm: 
-  assumes  "p\<in>nat" "l\<in>nat" "q\<in>nat" "t1\<in>nat" "t2\<in>nat"  "env\<in>list(M)" 
-  shows "sats(M,forces_eq_fm(p,l,q,t1,t2),env) \<longleftrightarrow> 
+lemma sats_forces_eq'_fm:
+  assumes  "p\<in>nat" "l\<in>nat" "q\<in>nat" "t1\<in>nat" "t2\<in>nat"  "env\<in>list(M)"
+  shows "sats(M,forces_eq_fm(p,l,q,t1,t2),env) \<longleftrightarrow>
          is_forces_eq'(##M,nth(p,env),nth(l,env),nth(q,env),nth(t1,env),nth(t2,env))"
   unfolding forces_eq_fm_def is_forces_eq'_def using assms sats_is_tuple_fm  sats_frc_at_fm
   by simp
 
-lemma sats_forces_mem'_fm: 
+lemma sats_forces_mem'_fm:
   assumes  "p\<in>nat" "l\<in>nat" "q\<in>nat" "t1\<in>nat" "t2\<in>nat"  "env\<in>list(M)"
-  shows "sats(M,forces_mem_fm(p,l,q,t1,t2),env) \<longleftrightarrow> 
+  shows "sats(M,forces_mem_fm(p,l,q,t1,t2),env) \<longleftrightarrow>
              is_forces_mem'(##M,nth(p,env),nth(l,env),nth(q,env),nth(t1,env),nth(t2,env))"
   unfolding forces_mem_fm_def is_forces_mem'_def using assms sats_is_tuple_fm sats_frc_at_fm
   by simp
 
-lemma sats_forces_neq'_fm: 
+lemma sats_forces_neq'_fm:
   assumes  "p\<in>nat" "l\<in>nat" "q\<in>nat" "t1\<in>nat" "t2\<in>nat"  "env\<in>list(M)"
-  shows "sats(M,forces_neq_fm(p,l,q,t1,t2),env) \<longleftrightarrow> 
+  shows "sats(M,forces_neq_fm(p,l,q,t1,t2),env) \<longleftrightarrow>
              is_forces_neq'(##M,nth(p,env),nth(l,env),nth(q,env),nth(t1,env),nth(t2,env))"
-  unfolding forces_neq_fm_def is_forces_neq'_def 
+  unfolding forces_neq_fm_def is_forces_neq'_def
   using assms sats_forces_eq'_fm sats_is_tuple_fm sats_frc_at_fm
   by simp
 
-lemma sats_forces_nmem'_fm: 
+lemma sats_forces_nmem'_fm:
   assumes  "p\<in>nat" "l\<in>nat" "q\<in>nat" "t1\<in>nat" "t2\<in>nat"  "env\<in>list(M)"
-  shows "sats(M,forces_nmem_fm(p,l,q,t1,t2),env) \<longleftrightarrow> 
+  shows "sats(M,forces_nmem_fm(p,l,q,t1,t2),env) \<longleftrightarrow>
              is_forces_nmem'(##M,nth(p,env),nth(l,env),nth(q,env),nth(t1,env),nth(t2,env))"
-  unfolding forces_nmem_fm_def is_forces_nmem'_def 
+  unfolding forces_nmem_fm_def is_forces_nmem'_def
   using assms sats_forces_mem'_fm sats_is_tuple_fm sats_frc_at_fm
   by simp
 
@@ -695,14 +695,14 @@ lemma cond_of_abs[simp]:
   by (rule hcomp_abs[OF snd_abs snd_snd_abs];simp_all add:fst_snd_closed)
 
 lemma tuple_abs[simp]:
-  "\<lbrakk>z\<in>M;t1\<in>M;t2\<in>M;p\<in>M;t\<in>M\<rbrakk> \<Longrightarrow> 
-   is_tuple(##M,z,t1,t2,p,t) \<longleftrightarrow> t = <z,t1,t2,p>" 
+  "\<lbrakk>z\<in>M;t1\<in>M;t2\<in>M;p\<in>M;t\<in>M\<rbrakk> \<Longrightarrow>
+   is_tuple(##M,z,t1,t2,p,t) \<longleftrightarrow> t = <z,t1,t2,p>"
   unfolding is_tuple_def using tuples_in_M by simp
 
 lemma oneN_in_M[simp]: "1\<in>M"
   by (simp flip: setclass_iff)
 
-lemma twoN_in_M : "2\<in>M" 
+lemma twoN_in_M : "2\<in>M"
   by (simp flip: setclass_iff)
 
 lemma comp_in_M:
@@ -714,7 +714,7 @@ lemma comp_in_M:
 
 lemma eq_case_abs [simp]:
   assumes
-    "t1\<in>M" "t2\<in>M" "p\<in>M" "f\<in>M" 
+    "t1\<in>M" "t2\<in>M" "p\<in>M" "f\<in>M"
   shows
     "is_eq_case(##M,t1,t2,p,P,leq,f) \<longleftrightarrow> eq_case(t1,t2,p,P,leq,f)"
 proof -
@@ -724,34 +724,71 @@ proof -
   have "\<langle>s,y\<rangle>\<in>t \<Longrightarrow> s\<in>domain(t)" if "t\<in>M" for s y t
     using that unfolding domain_def by auto
   ultimately
-  have 
-    "(\<forall>s\<in>M. s \<in> domain(t1) \<or> s \<in> domain(t2) \<longrightarrow> (\<forall>q\<in>M. q\<in>P \<and> q \<preceq> p \<longrightarrow> 
+  have
+    "(\<forall>s\<in>M. s \<in> domain(t1) \<or> s \<in> domain(t2) \<longrightarrow> (\<forall>q\<in>M. q\<in>P \<and> q \<preceq> p \<longrightarrow>
                               (f ` \<langle>1, s, t1, q\<rangle> =1 \<longleftrightarrow> f ` \<langle>1, s, t2, q\<rangle>=1))) \<longleftrightarrow>
-    (\<forall>s. s \<in> domain(t1) \<or> s \<in> domain(t2) \<longrightarrow> (\<forall>q. q\<in>P \<and> q \<preceq> p \<longrightarrow> 
-                                  (f ` \<langle>1, s, t1, q\<rangle> =1 \<longleftrightarrow> f ` \<langle>1, s, t2, q\<rangle>=1)))" 
-    using assms domain_trans[OF trans_M,of t1] 
+    (\<forall>s. s \<in> domain(t1) \<or> s \<in> domain(t2) \<longrightarrow> (\<forall>q. q\<in>P \<and> q \<preceq> p \<longrightarrow>
+                                  (f ` \<langle>1, s, t1, q\<rangle> =1 \<longleftrightarrow> f ` \<langle>1, s, t2, q\<rangle>=1)))"
+    using assms domain_trans[OF trans_M,of t1]
       domain_trans[OF trans_M,of t2] by auto
   then show ?thesis
-    unfolding eq_case_def is_eq_case_def 
-    using assms pair_in_M_iff n_in_M[of 1] domain_closed tuples_in_M 
+    unfolding eq_case_def is_eq_case_def
+    using assms pair_in_M_iff n_in_M[of 1] domain_closed tuples_in_M
       apply_closed leq_in_M
     by simp
 qed
 
 lemma mem_case_abs [simp]:
   assumes
-    "t1\<in>M" "t2\<in>M" "p\<in>M" "f\<in>M" 
+    "t1\<in>M" "t2\<in>M" "p\<in>M" "f\<in>M"
   shows
     "is_mem_case(##M,t1,t2,p,P,leq,f) \<longleftrightarrow> mem_case(t1,t2,p,P,leq,f)"
-  unfolding is_mem_case_def mem_case_def using assms zero_in_M pair_in_M_iff
-    comp_in_M 
-  apply auto 
-   apply blast
-  apply (drule bspec,auto)
-  apply (rule bexI)+
-     defer 1 prefer 2
-     apply (rule domain_trans[OF trans_M,of t2],auto)
-  done
+proof
+  {
+    fix v
+    assume "v\<in>P" "v \<preceq> p" "is_mem_case(##M,t1,t2,p,P,leq,f)"
+    moreover
+    from this
+    have "v\<in>M" "\<langle>v,p\<rangle> \<in> M" "(##M)(v)"
+      using transitivity[OF _ P_in_M,of v] transitivity[OF _ leq_in_M]
+      by simp_all
+    moreover
+    from calculation assms
+    obtain q r s where
+      "r \<in> P \<and> q \<in> P \<and> \<langle>q, v\<rangle> \<in> M \<and> \<langle>s, r\<rangle> \<in> M \<and> \<langle>q, r\<rangle> \<in> M \<and> 0 \<in> M \<and>
+       \<langle>0, t1, s, q\<rangle> \<in> M \<and> q \<preceq> v \<and> \<langle>s, r\<rangle> \<in> t2 \<and> q \<preceq> r \<and> f ` \<langle>0, t1, s, q\<rangle> = 1"
+      unfolding is_mem_case_def by auto
+    then
+    have "\<exists>q s r. r \<in> P \<and> q \<in> P \<and> q \<preceq> v \<and> \<langle>s, r\<rangle> \<in> t2 \<and> q \<preceq> r \<and> f ` \<langle>0, t1, s, q\<rangle> = 1"
+      by auto
+  }
+  then
+  show "mem_case(t1, t2, p, P, leq, f)" if "is_mem_case(##M, t1, t2, p, P, leq, f)"
+    unfolding mem_case_def using that assms by auto
+next
+  { fix v
+    assume "v \<in> M" "v \<in> P" "\<langle>v, p\<rangle> \<in> M" "v \<preceq> p" "mem_case(t1, t2, p, P, leq, f)"
+    moreover
+    from this
+    obtain q s r where "r \<in> P \<and> q \<in> P \<and> q \<preceq> v \<and> \<langle>s, r\<rangle> \<in> t2 \<and> q \<preceq> r \<and> f ` \<langle>0, t1, s, q\<rangle> = 1"
+      unfolding mem_case_def by auto
+    moreover
+    from this \<open>t2\<in>M\<close>
+    have "r\<in>M" "q\<in>M" "s\<in>M" "r \<in> P \<and> q \<in> P \<and> q \<preceq> v \<and> \<langle>s, r\<rangle> \<in> t2 \<and> q \<preceq> r \<and> f ` \<langle>0, t1, s, q\<rangle> = 1"
+      using transitivity P_in_M domain_closed[of t2] by auto
+    moreover
+    note \<open>t1\<in>M\<close>
+    ultimately
+    have "\<exists>q\<in>M . \<exists>s\<in>M. \<exists>r\<in>M.
+         r \<in> P \<and> q \<in> P \<and> \<langle>q, v\<rangle> \<in> M \<and> \<langle>s, r\<rangle> \<in> M \<and> \<langle>q, r\<rangle> \<in> M \<and> 0 \<in> M \<and>
+         \<langle>0, t1, s, q\<rangle> \<in> M \<and> q \<preceq> v \<and> \<langle>s, r\<rangle> \<in> t2 \<and> q \<preceq> r \<and> f ` \<langle>0, t1, s, q\<rangle> = 1"
+      using tuples_in_M zero_in_M by auto
+  }
+  then
+  show "is_mem_case(##M, t1, t2, p, P, leq, f)" if "mem_case(t1, t2, p, P, leq, f)"
+    unfolding is_mem_case_def using assms that by auto
+qed
+
 
 lemma Hfrc_abs:
   "\<lbrakk>fnnc\<in>M; f\<in>M\<rbrakk> \<Longrightarrow>
@@ -789,13 +826,13 @@ lemma is_eclose_n_abs :
 
 
 lemma is_ecloseN_abs :
-  "\<lbrakk>x\<in>M;ec\<in>M\<rbrakk> \<Longrightarrow> is_ecloseN(##M,ec,x) \<longleftrightarrow> ec = ecloseN(x)" 
-  unfolding is_ecloseN_def ecloseN_def 
+  "\<lbrakk>x\<in>M;ec\<in>M\<rbrakk> \<Longrightarrow> is_ecloseN(##M,ec,x) \<longleftrightarrow> ec = ecloseN(x)"
+  unfolding is_ecloseN_def ecloseN_def
   using is_eclose_n_abs Un_closed union_abs ecloseN_closed
   by auto
 
 lemma frecR_abs :
-  "x\<in>M \<Longrightarrow> y\<in>M \<Longrightarrow> frecR(x,y) \<longleftrightarrow> is_frecR(##M,x,y)" 
+  "x\<in>M \<Longrightarrow> y\<in>M \<Longrightarrow> frecR(x,y) \<longleftrightarrow> is_frecR(##M,x,y)"
   unfolding frecR_def is_frecR_def using components_closed domain_closed by simp
 
 lemma frecrelP_abs :
@@ -803,7 +840,7 @@ lemma frecrelP_abs :
   using pair_in_M_iff frecR_abs unfolding frecrelP_def by auto
 
 lemma frecrel_abs:
-  assumes 
+  assumes
     "A\<in>M" "r\<in>M"
   shows
     "is_frecrel(##M,A,r) \<longleftrightarrow>  r = frecrel(A)"
@@ -820,14 +857,14 @@ proof -
 qed
 
 lemma frecrel_closed:
-  assumes 
-    "x\<in>M" 
+  assumes
+    "x\<in>M"
   shows
-    "frecrel(x)\<in>M" 
+    "frecrel(x)\<in>M"
 proof -
   have "Collect(x\<times>x,\<lambda>z. (\<exists>x y. z = <x,y> \<and> frecR(x,y)))\<in>M"
     using Collect_in_M_0p[of "frecrelP_fm(0)"] arity_frecrelP_fm sats_frecrelP_fm
-      frecrelP_abs \<open>x\<in>M\<close> cartprod_closed by simp 
+      frecrelP_abs \<open>x\<in>M\<close> cartprod_closed by simp
   then show ?thesis
     unfolding frecrel_def Rrel_def frecrelP_def by simp
 qed
@@ -847,31 +884,31 @@ lemma wf_forcerel :
 lemma restrict_trancl_forcerel:
   assumes "frecR(w,y)"
   shows "restrict(f,frecrel(names_below(P,x))-``{y})`w
-       = restrict(f,forcerel(P,x)-``{y})`w" 
-  unfolding forcerel_def frecrel_def using assms restrict_trancl_Rrel[of frecR] 
+       = restrict(f,forcerel(P,x)-``{y})`w"
+  unfolding forcerel_def frecrel_def using assms restrict_trancl_Rrel[of frecR]
   by simp
 
-lemma names_belowI : 
+lemma names_belowI :
   assumes "frecR(<ft,n1,n2,p>,<a,b,c,d>)" "p\<in>P"
   shows "<ft,n1,n2,p> \<in> names_below(P,<a,b,c,d>)" (is "?x \<in> names_below(_,?y)")
 proof -
   from assms
-  have "ft \<in> 2" "a \<in> 2" 
+  have "ft \<in> 2" "a \<in> 2"
     unfolding frecR_def by (auto simp add:components_simp)
   from assms
-  consider (e) "n1 \<in> domain(b) \<union> domain(c) \<and> (n2 = b \<or> n2 =c)" 
+  consider (e) "n1 \<in> domain(b) \<union> domain(c) \<and> (n2 = b \<or> n2 =c)"
     | (m) "n1 = b \<and> n2 \<in> domain(c)"
     unfolding frecR_def by (auto simp add:components_simp)
-  then show ?thesis 
+  then show ?thesis
   proof cases
     case e
-    then 
-    have "n1 \<in> eclose(b) \<or> n1 \<in> eclose(c)"  
+    then
+    have "n1 \<in> eclose(b) \<or> n1 \<in> eclose(c)"
       using Un_iff in_dom_in_eclose by auto
     with e
     have "n1 \<in> ecloseN(?y)" "n2 \<in> ecloseN(?y)"
       using ecloseNI components_in_eclose by auto
-    with \<open>ft\<in>2\<close> \<open>p\<in>P\<close> 
+    with \<open>ft\<in>2\<close> \<open>p\<in>P\<close>
     show ?thesis unfolding names_below_def by  auto
   next
     case m
@@ -879,14 +916,14 @@ proof -
     have "n1 \<in> ecloseN(?y)" "n2 \<in> ecloseN(?y)"
       using mem_eclose_trans  ecloseNI
         in_dom_in_eclose components_in_eclose by auto
-    with \<open>ft\<in>2\<close> \<open>p\<in>P\<close> 
+    with \<open>ft\<in>2\<close> \<open>p\<in>P\<close>
     show ?thesis unfolding names_below_def
-      by auto    
+      by auto
   qed
 qed
 
-lemma names_below_tr : 
-  assumes "x\<in> names_below(P,y)" 
+lemma names_below_tr :
+  assumes "x\<in> names_below(P,y)"
     "y\<in> names_below(P,z)"
   shows "x\<in> names_below(P,z)"
 proof -
@@ -903,7 +940,7 @@ proof -
   have "x1\<in>ecloseN(z)" "x2\<in>ecloseN(z)"
     using ecloseN_mono names_simp by auto
   with \<open>fx\<in>2\<close> \<open>px\<in>P\<close> \<open>x=_\<close>
-  have "x\<in>?A(z)" 
+  have "x\<in>?A(z)"
     unfolding names_below_def by simp
   then show ?thesis using subsetI by simp
 qed
@@ -918,7 +955,7 @@ proof -
       unfolding frecrel_def Rrel_def
       by auto
     obtain f n1 n2 p where
-      "x = <f,n1,n2,p>" "f\<in>2" "n1\<in>ecloseN(z)" "n2\<in>ecloseN(z)" "p\<in>P" 
+      "x = <f,n1,n2,p>" "f\<in>2" "n1\<in>ecloseN(z)" "n2\<in>ecloseN(z)" "p\<in>P"
       using \<open>x\<in>names_below(P,z)\<close>
       unfolding names_below_def by auto
     moreover
@@ -926,9 +963,9 @@ proof -
       "q\<in>P" "y = <fy,m1,m2,q>"
       using \<open>y\<in>names_below(P,z)\<close>
       unfolding names_below_def by auto
-    moreover 
+    moreover
     note \<open>frecR(x,y)\<close>
-    ultimately 
+    ultimately
     have "x\<in>names_below(P,y)" using names_belowI by simp
   }
   then show ?thesis .
@@ -943,15 +980,15 @@ proof -
     have "x\<in>names_below(P,z)"
       unfolding frecrel_def Rrel_def
       by auto
-    from \<open>x\<in>names_below(P,z)\<close> 
+    from \<open>x\<in>names_below(P,z)\<close>
     obtain f n1 n2 p where
       "x = <f,n1,n2,p>" "f\<in>2" "n1\<in>ecloseN(z)" "n2\<in>ecloseN(z)" "p\<in>P"
       unfolding names_below_def by auto
     then
-    have "n1\<in>ecloseN(x)" "n2\<in>ecloseN(x)" 
+    have "n1\<in>ecloseN(x)" "n2\<in>ecloseN(x)"
       using components_in_eclose by simp_all
     with \<open>f\<in>2\<close> \<open>p\<in>P\<close> \<open>x = <f,n1,n2,p>\<close>
-    have "x\<in>names_below(P,x)" 
+    have "x\<in>names_below(P,x)"
       unfolding names_below_def by simp
   }
   then show ?thesis .
@@ -964,50 +1001,50 @@ lemma forcerel_arg_into_names_below :
   unfolding forcerel_def
   by(rule trancl_induct;auto simp add: arg_into_names_below)
 
-lemma names_below_mono : 
+lemma names_below_mono :
   assumes "\<langle>x,y\<rangle> \<in> frecrel(names_below(P,z))"
   shows "names_below(P,x) \<subseteq> names_below(P,y)"
 proof -
   from assms
   have "x\<in>names_below(P,y)"
     using arg_into_names_below2 by simp
-  then 
-  show ?thesis 
+  then
+  show ?thesis
     using names_below_tr subsetI by simp
 qed
 
-lemma frecrel_mono : 
+lemma frecrel_mono :
   assumes "\<langle>x,y\<rangle> \<in> frecrel(names_below(P,z))"
   shows "frecrel(names_below(P,x)) \<subseteq> frecrel(names_below(P,y))"
   unfolding frecrel_def
   using Rrel_mono names_below_mono assms by simp
 
-lemma forcerel_mono2 : 
+lemma forcerel_mono2 :
   assumes "\<langle>x,y\<rangle> \<in> frecrel(names_below(P,z))"
   shows "forcerel(P,x) \<subseteq> forcerel(P,y)"
   unfolding forcerel_def
   using trancl_mono frecrel_mono assms by simp
 
-lemma forcerel_mono_aux : 
+lemma forcerel_mono_aux :
   assumes "\<langle>x,y\<rangle> \<in> frecrel(names_below(P, w))^+"
   shows "forcerel(P,x) \<subseteq> forcerel(P,y)"
-  using assms 
+  using assms
   by (rule trancl_induct,simp_all add: subset_trans forcerel_mono2)
 
-lemma forcerel_mono : 
+lemma forcerel_mono :
   assumes "\<langle>x,y\<rangle> \<in> forcerel(P,z)"
   shows "forcerel(P,x) \<subseteq> forcerel(P,y)"
   using forcerel_mono_aux assms unfolding forcerel_def by simp
 
-lemma aux: "x \<in> names_below(P, w) \<Longrightarrow> <x,y> \<in> forcerel(P,z) \<Longrightarrow> 
+lemma aux: "x \<in> names_below(P, w) \<Longrightarrow> <x,y> \<in> forcerel(P,z) \<Longrightarrow>
   (y \<in> names_below(P, w) \<longrightarrow> <x,y> \<in> forcerel(P,w))"
   unfolding forcerel_def
 proof(rule_tac a=x and b=y and P="\<lambda> y . y \<in> names_below(P, w) \<longrightarrow> <x,y> \<in> frecrel(names_below(P,w))^+" in trancl_induct,simp)
   let ?A="\<lambda> a . names_below(P, a)"
   let ?R="\<lambda> a . frecrel(?A(a))"
-  let ?fR="\<lambda> a .forcerel(a)"  
-  show "u\<in>?A(w) \<longrightarrow> <x,u>\<in>?R(w)^+" if "x\<in>?A(w)" "<x,y>\<in>?R(z)^+" "<x,u>\<in>?R(z)"  for  u 
-    using that frecrelD frecrelI r_into_trancl unfolding names_below_def by simp  
+  let ?fR="\<lambda> a .forcerel(a)"
+  show "u\<in>?A(w) \<longrightarrow> <x,u>\<in>?R(w)^+" if "x\<in>?A(w)" "<x,y>\<in>?R(z)^+" "<x,u>\<in>?R(z)"  for  u
+    using that frecrelD frecrelI r_into_trancl unfolding names_below_def by simp
   {
     fix u v
     assume "x \<in> ?A(w)"
@@ -1015,7 +1052,7 @@ proof(rule_tac a=x and b=y and P="\<lambda> y . y \<in> names_below(P, w) \<long
       "\<langle>x, u\<rangle> \<in> ?R(z)^+"
       "\<langle>u, v\<rangle> \<in> ?R(z)"
       "u \<in> ?A(w) \<Longrightarrow> \<langle>x, u\<rangle> \<in> ?R(w)^+"
-    then 
+    then
     have "v \<in> ?A(w) \<Longrightarrow> \<langle>x, v\<rangle> \<in> ?R(w)^+"
     proof -
       assume "v \<in>?A(w)"
@@ -1026,7 +1063,7 @@ proof(rule_tac a=x and b=y and P="\<lambda> y . y \<in> names_below(P, w) \<long
       have "u\<in>?A(w)"
         using names_below_tr by simp
       with \<open>v\<in>_\<close> \<open>\<langle>u,v\<rangle>\<in>_\<close>
-      have "\<langle>u,v\<rangle>\<in> ?R(w)" 
+      have "\<langle>u,v\<rangle>\<in> ?R(w)"
         using frecrelD frecrelI r_into_trancl unfolding names_below_def by simp
       with \<open>u \<in> ?A(w) \<Longrightarrow> \<langle>x, u\<rangle> \<in> ?R(w)^+\<close> \<open>u\<in>?A(w)\<close>
       have "\<langle>x, u\<rangle> \<in> ?R(w)^+" by simp
@@ -1035,7 +1072,7 @@ proof(rule_tac a=x and b=y and P="\<lambda> y . y \<in> names_below(P, w) \<long
         by simp
     qed
   }
-  then show "v \<in> ?A(w) \<longrightarrow> \<langle>x, v\<rangle> \<in> ?R(w)^+" 
+  then show "v \<in> ?A(w) \<longrightarrow> \<langle>x, v\<rangle> \<in> ?R(w)^+"
     if "x \<in> ?A(w)"
       "\<langle>x, y\<rangle> \<in> ?R(z)^+"
       "\<langle>x, u\<rangle> \<in> ?R(z)^+"
@@ -1044,22 +1081,22 @@ proof(rule_tac a=x and b=y and P="\<lambda> y . y \<in> names_below(P, w) \<long
     using that by simp
 qed
 
-lemma forcerel_eq : 
+lemma forcerel_eq :
   assumes "\<langle>z,x\<rangle> \<in> forcerel(P,x)"
   shows "forcerel(P,z) = forcerel(P,x) \<inter> names_below(P,z)\<times>names_below(P,z)"
-  using assms aux forcerelD forcerel_mono[of z x x] subsetI 
+  using assms aux forcerelD forcerel_mono[of z x x] subsetI
   by auto
 
 lemma forcerel_below_aux :
   assumes "<z,x> \<in> forcerel(P,x)" "<u,z> \<in> forcerel(P,x)"
-  shows "u \<in> names_below(P,z)" 
+  shows "u \<in> names_below(P,z)"
   using assms(2)
   unfolding forcerel_def
 proof(rule trancl_induct)
   show  "u \<in> names_below(P,y)" if " \<langle>u, y\<rangle> \<in> frecrel(names_below(P, x))" for y
     using that vimage_singleton_iff arg_into_names_below2 by simp
 next
-  show "u \<in> names_below(P,z)" 
+  show "u \<in> names_below(P,z)"
     if "\<langle>u, y\<rangle> \<in> frecrel(names_below(P, x))^+"
       "\<langle>y, z\<rangle> \<in> frecrel(names_below(P, x))"
       "u \<in> names_below(P, y)"
@@ -1068,11 +1105,11 @@ next
 qed
 
 lemma forcerel_below :
-  assumes "<z,x> \<in> forcerel(P,x)" 
-  shows "forcerel(P,x) -`` {z} \<subseteq> names_below(P,z)" 
+  assumes "<z,x> \<in> forcerel(P,x)"
+  shows "forcerel(P,x) -`` {z} \<subseteq> names_below(P,z)"
   using vimage_singleton_iff assms forcerel_below_aux by auto
 
-lemma relation_forcerel : 
+lemma relation_forcerel :
   shows "relation(forcerel(P,z))" "trans(forcerel(P,z))"
   unfolding forcerel_def using relation_trancl trans_trancl by simp_all
 
@@ -1088,7 +1125,7 @@ lemma frc_at_trancl: "frc_at(P,leq,z) = wfrec(forcerel(P,z),z,\<lambda>x f. bool
   unfolding frc_at_def forcerel_def using wf_eq_trancl Hfrc_restrict_trancl by simp
 
 
-lemma forcerelI1 : 
+lemma forcerelI1 :
   assumes "n1 \<in> domain(b) \<or> n1 \<in> domain(c)" "p\<in>P" "d\<in>P"
   shows "\<langle>\<langle>1, n1, b, p\<rangle>, \<langle>0,b,c,d\<rangle>\<rangle>\<in> forcerel(P,\<langle>0,b,c,d\<rangle>)"
 proof -
@@ -1099,7 +1136,7 @@ proof -
     using frecRI1 by simp
   then
   have "?x\<in>names_below(P,?y)"  "?y \<in> names_below(P,?y)"
-    using names_belowI  assms components_in_eclose 
+    using names_belowI  assms components_in_eclose
     unfolding names_below_def by auto
   with \<open>frecR(?x,?y)\<close>
   show ?thesis
@@ -1108,7 +1145,7 @@ proof -
     by auto
 qed
 
-lemma forcerelI2 : 
+lemma forcerelI2 :
   assumes "n1 \<in> domain(b) \<or> n1 \<in> domain(c)" "p\<in>P" "d\<in>P"
   shows "\<langle>\<langle>1, n1, c, p\<rangle>, \<langle>0,b,c,d\<rangle>\<rangle>\<in> forcerel(P,\<langle>0,b,c,d\<rangle>)"
 proof -
@@ -1119,16 +1156,16 @@ proof -
     using frecRI2 by simp
   then
   have "?x\<in>names_below(P,?y)"  "?y \<in> names_below(P,?y)"
-    using names_belowI  assms components_in_eclose 
+    using names_belowI  assms components_in_eclose
     unfolding names_below_def by auto
   with \<open>frecR(?x,?y)\<close>
   show ?thesis
-    unfolding forcerel_def frecrel_def 
+    unfolding forcerel_def frecrel_def
     using subsetD[OF r_subset_trancl[OF relation_Rrel]] RrelI
     by auto
 qed
 
-lemma forcerelI3 : 
+lemma forcerelI3 :
   assumes "\<langle>n2, r\<rangle> \<in> c" "p\<in>P" "d\<in>P" "r \<in> P"
   shows "\<langle>\<langle>0, b, n2, p\<rangle>,\<langle>1, b, c, d\<rangle>\<rangle> \<in> forcerel(P,<1,b,c,d>)"
 proof -
@@ -1139,16 +1176,16 @@ proof -
     using assms frecRI3 by simp
   then
   have "?x\<in>names_below(P,?y)"  "?y \<in> names_below(P,?y)"
-    using names_belowI  assms components_in_eclose 
+    using names_belowI  assms components_in_eclose
     unfolding names_below_def by auto
   with \<open>frecR(?x,?y)\<close>
   show ?thesis
-    unfolding forcerel_def frecrel_def 
+    unfolding forcerel_def frecrel_def
     using subsetD[OF r_subset_trancl[OF relation_Rrel]] RrelI
     by auto
 qed
 
-lemmas forcerelI = forcerelI1[THEN vimage_singleton_iff[THEN iffD2]] 
+lemmas forcerelI = forcerelI1[THEN vimage_singleton_iff[THEN iffD2]]
   forcerelI2[THEN vimage_singleton_iff[THEN iffD2]]
   forcerelI3[THEN vimage_singleton_iff[THEN iffD2]]
 
@@ -1158,49 +1195,49 @@ lemma  aux_def_frc_at:
 proof -
   let ?A="names_below(P,z)"
   from assms
-  have "<z,x> \<in> forcerel(P,x)" 
+  have "<z,x> \<in> forcerel(P,x)"
     using vimage_singleton_iff by simp
-  then 
-  have "z \<in> ?A" 
+  then
+  have "z \<in> ?A"
     using forcerel_arg_into_names_below by simp
   from \<open><z,x> \<in> forcerel(P,x)\<close>
   have E:"forcerel(P,z) = forcerel(P,x) \<inter> (?A\<times>?A)"
-    "forcerel(P,x) -`` {z} \<subseteq> ?A" 
+    "forcerel(P,x) -`` {z} \<subseteq> ?A"
     using forcerel_eq forcerel_below
     by auto
   with \<open>z\<in>?A\<close>
   have "wfrec(forcerel(P,x), z, H) = wfrec[?A](forcerel(P,x), z, H)"
     using wfrec_trans_restr[OF relation_forcerel(1) wf_forcerel relation_forcerel(2), of x z ?A]
     by simp
-  then show ?thesis 
+  then show ?thesis
     using E wfrec_restr_eq by simp
 qed
 
 subsection\<open>Recursive expression of \<^term>\<open>frc_at\<close>\<close>
 
-lemma def_frc_at : 
+lemma def_frc_at :
   assumes "p\<in>P"
   shows
     "frc_at(P,leq,<ft,n1,n2,p>) =
-   bool_of_o( p \<in>P \<and> 
+   bool_of_o( p \<in>P \<and>
   (  ft = 0 \<and>  (\<forall>s. s\<in>domain(n1) \<union> domain(n2) \<longrightarrow>
         (\<forall>q. q\<in>P \<and> q \<preceq> p \<longrightarrow> (frc_at(P,leq,<1,s,n1,q>) =1 \<longleftrightarrow> frc_at(P,leq,<1,s,n2,q>) =1)))
    \<or> ft = 1 \<and> ( \<forall>v\<in>P. v \<preceq> p \<longrightarrow>
     (\<exists>q. \<exists>s. \<exists>r. r\<in>P \<and> q\<in>P \<and> q \<preceq> v \<and> <s,r> \<in> n2 \<and> q \<preceq> r \<and>  frc_at(P,leq,<0,n1,s,q>) = 1))))"
 proof -
   let ?r="\<lambda>y. forcerel(P,y)" and ?Hf="\<lambda>x f. bool_of_o(Hfrc(P,leq,x,f))"
-  let ?t="\<lambda>y. ?r(y) -`` {y}" 
+  let ?t="\<lambda>y. ?r(y) -`` {y}"
   let ?arg="<ft,n1,n2,p>"
-  from wf_forcerel 
+  from wf_forcerel
   have wfr: "\<forall>w . wf(?r(w))" ..
-  with wfrec [of "?r(?arg)" ?arg ?Hf] 
+  with wfrec [of "?r(?arg)" ?arg ?Hf]
   have "frc_at(P,leq,?arg) = ?Hf( ?arg, \<lambda>x\<in>?r(?arg) -`` {?arg}. wfrec(?r(?arg), x, ?Hf))"
-    using frc_at_trancl by simp 
+    using frc_at_trancl by simp
   also
   have " ... = ?Hf( ?arg, \<lambda>x\<in>?r(?arg) -`` {?arg}. frc_at(P,leq,x))"
     using aux_def_frc_at frc_at_trancl by simp
-  finally 
-  show ?thesis  
+  finally
+  show ?thesis
     unfolding Hfrc_def mem_case_def eq_case_def
     using forcerelI  assms
     by auto
@@ -1212,15 +1249,15 @@ subsection\<open>Absoluteness of \<^term>\<open>frc_at\<close>\<close>
 lemma trans_forcerel_t : "trans(forcerel(P,x))"
   unfolding forcerel_def using trans_trancl .
 
-lemma relation_forcerel_t : "relation(forcerel(P,x))" 
+lemma relation_forcerel_t : "relation(forcerel(P,x))"
   unfolding forcerel_def using relation_trancl .
 
 
 lemma forcerel_in_M :
-  assumes 
-    "x\<in>M" 
-  shows 
-    "forcerel(P,x)\<in>M" 
+  assumes
+    "x\<in>M"
+  shows
+    "forcerel(P,x)\<in>M"
   unfolding forcerel_def def_frecrel names_below_def
 proof -
   let ?Q = "2 \<times> ecloseN(x) \<times> ecloseN(x) \<times> P"
@@ -1230,26 +1267,26 @@ proof -
   have "separation(##M,\<lambda>z. \<exists>x y. z = \<langle>x, y\<rangle> \<and> frecR(x, y))"
   proof -
     have "arity(frecrelP_fm(0)) = 1"
-      unfolding number1_fm_def frecrelP_fm_def 
+      unfolding number1_fm_def frecrelP_fm_def
       by (simp del:FOL_sats_iff pair_abs empty_abs
           add: fm_defs frecR_fm_def number1_fm_def components_defs nat_simp_union)
     then
     have "separation(##M, \<lambda>z. sats(M,frecrelP_fm(0) , [z]))"
       using separation_ax by simp
     moreover
-    have "frecrelP(##M,z) \<longleftrightarrow> sats(M,frecrelP_fm(0),[z])" 
+    have "frecrelP(##M,z) \<longleftrightarrow> sats(M,frecrelP_fm(0),[z])"
       if "z\<in>M" for z
       using that sats_frecrelP_fm[of 0 "[z]"] by simp
     ultimately
-    have "separation(##M,frecrelP(##M))" 
+    have "separation(##M,frecrelP(##M))"
       unfolding separation_def by simp
-    then 
+    then
     show ?thesis using frecrelP_abs
         separation_cong[of "##M" "frecrelP(##M)" "\<lambda>z. \<exists>x y. z = \<langle>x, y\<rangle> \<and> frecR(x, y)"]
       by simp
   qed
   ultimately
-  show "{z \<in> ?Q \<times> ?Q . \<exists>x y. z = \<langle>x, y\<rangle> \<and> frecR(x, y)}^+ \<in> M" 
+  show "{z \<in> ?Q \<times> ?Q . \<exists>x y. z = \<langle>x, y\<rangle> \<and> frecR(x, y)}^+ \<in> M"
     using separation_closed frecrelP_abs trancl_closed by simp
 qed
 
@@ -1259,41 +1296,41 @@ lemma relation2_Hfrc_at_abs:
   by simp
 
 lemma Hfrc_at_closed :
-  "\<forall>x\<in>M. \<forall>g\<in>M. function(g) \<longrightarrow> bool_of_o(Hfrc(P,leq,x,g))\<in>M" 
+  "\<forall>x\<in>M. \<forall>g\<in>M. function(g) \<longrightarrow> bool_of_o(Hfrc(P,leq,x,g))\<in>M"
   unfolding bool_of_o_def using zero_in_M n_in_M[of 1] by simp
 
 lemma wfrec_Hfrc_at :
   assumes
-    "X\<in>M" 
-  shows 
+    "X\<in>M"
+  shows
     "wfrec_replacement(##M,is_Hfrc_at(##M,P,leq),forcerel(P,X))"
 proof -
-  have 0:"is_Hfrc_at(##M,P,leq,a,b,c) \<longleftrightarrow> 
+  have 0:"is_Hfrc_at(##M,P,leq,a,b,c) \<longleftrightarrow>
         sats(M,Hfrc_at_fm(8,9,2,1,0),[c,b,a,d,e,y,x,z,P,leq,forcerel(P,X)])"
-    if "a\<in>M" "b\<in>M" "c\<in>M" "d\<in>M" "e\<in>M" "y\<in>M" "x\<in>M" "z\<in>M" 
+    if "a\<in>M" "b\<in>M" "c\<in>M" "d\<in>M" "e\<in>M" "y\<in>M" "x\<in>M" "z\<in>M"
     for a b c d e y x z
-    using that P_in_M leq_in_M \<open>X\<in>M\<close> forcerel_in_M 
-      is_Hfrc_at_iff_sats[of concl:M P leq a b c 8 9 2 1 0 
+    using that P_in_M leq_in_M \<open>X\<in>M\<close> forcerel_in_M
+      is_Hfrc_at_iff_sats[of concl:M P leq a b c 8 9 2 1 0
         "[c,b,a,d,e,y,x,z,P,leq,forcerel(P,X)]"] by simp
   have 1:"sats(M,is_wfrec_fm(Hfrc_at_fm(8,9,2,1,0),5,1,0),[y,x,z,P,leq,forcerel(P,X)]) \<longleftrightarrow>
                    is_wfrec(##M, is_Hfrc_at(##M,P,leq),forcerel(P,X), x, y)"
     if "x\<in>M" "y\<in>M" "z\<in>M" for x y z
     using  that \<open>X\<in>M\<close> forcerel_in_M P_in_M leq_in_M
-      sats_is_wfrec_fm[OF 0] 
+      sats_is_wfrec_fm[OF 0]
     by simp
-  let 
+  let
     ?f="Exists(And(pair_fm(1,0,2),is_wfrec_fm(Hfrc_at_fm(8,9,2,1,0),5,1,0)))"
   have satsf:"sats(M, ?f, [x,z,P,leq,forcerel(P,X)]) \<longleftrightarrow>
-              (\<exists>y\<in>M. pair(##M,x,y,z) & is_wfrec(##M, is_Hfrc_at(##M,P,leq),forcerel(P,X), x, y))" 
+              (\<exists>y\<in>M. pair(##M,x,y,z) & is_wfrec(##M, is_Hfrc_at(##M,P,leq),forcerel(P,X), x, y))"
     if "x\<in>M" "z\<in>M" for x z
     using that 1 \<open>X\<in>M\<close> forcerel_in_M P_in_M leq_in_M by (simp del:pair_abs)
-  have artyf:"arity(?f) = 5" 
+  have artyf:"arity(?f) = 5"
     unfolding is_wfrec_fm_def Hfrc_at_fm_def Hfrc_fm_def Replace_fm_def PHcheck_fm_def
       pair_fm_def upair_fm_def is_recfun_fm_def fun_apply_fm_def big_union_fm_def
       pre_image_fm_def restriction_fm_def image_fm_def fm_defs number1_fm_def
       eq_case_fm_def mem_case_fm_def is_tuple_fm_def
     by (simp add:nat_simp_union)
-  moreover 
+  moreover
   have "?f\<in>formula"
     unfolding fm_defs Hfrc_at_fm_def by simp
   ultimately
@@ -1303,44 +1340,44 @@ proof -
   have "strong_replacement(##M,\<lambda>x z.
           \<exists>y\<in>M. pair(##M,x,y,z) & is_wfrec(##M, is_Hfrc_at(##M,P,leq),forcerel(P,X), x, y))"
     using repl_sats[of M ?f "[P,leq,forcerel(P,X)]"] satsf by (simp del:pair_abs)
-  then 
+  then
   show ?thesis unfolding wfrec_replacement_def by simp
 qed
 
 lemma names_below_abs :
-  "\<lbrakk>Q\<in>M;x\<in>M;nb\<in>M\<rbrakk> \<Longrightarrow> is_names_below(##M,Q,x,nb) \<longleftrightarrow> nb = names_below(Q,x)" 
-  unfolding is_names_below_def names_below_def 
-  using succ_in_M_iff zero_in_M cartprod_closed is_ecloseN_abs ecloseN_closed 
+  "\<lbrakk>Q\<in>M;x\<in>M;nb\<in>M\<rbrakk> \<Longrightarrow> is_names_below(##M,Q,x,nb) \<longleftrightarrow> nb = names_below(Q,x)"
+  unfolding is_names_below_def names_below_def
+  using succ_in_M_iff zero_in_M cartprod_closed is_ecloseN_abs ecloseN_closed
   by auto
 
 lemma names_below_closed:
   "\<lbrakk>Q\<in>M;x\<in>M\<rbrakk> \<Longrightarrow> names_below(Q,x) \<in> M"
-  unfolding names_below_def 
-  using zero_in_M cartprod_closed ecloseN_closed succ_in_M_iff 
+  unfolding names_below_def
+  using zero_in_M cartprod_closed ecloseN_closed succ_in_M_iff
   by simp
 
 lemma "names_below_productE" :
   assumes "Q \<in> M" "x \<in> M"
-   "\<And>A1 A2 A3 A4. A1 \<in> M \<Longrightarrow> A2 \<in> M \<Longrightarrow> A3 \<in> M \<Longrightarrow> A4 \<in> M \<Longrightarrow> R(A1 \<times> A2 \<times> A3 \<times> A4)"
- shows "R(names_below(Q,x))" 
+    "\<And>A1 A2 A3 A4. A1 \<in> M \<Longrightarrow> A2 \<in> M \<Longrightarrow> A3 \<in> M \<Longrightarrow> A4 \<in> M \<Longrightarrow> R(A1 \<times> A2 \<times> A3 \<times> A4)"
+  shows "R(names_below(Q,x))"
   unfolding names_below_def using assms zero_in_M ecloseN_closed[of x] twoN_in_M by auto
 
 lemma forcerel_abs :
-  "\<lbrakk>x\<in>M;z\<in>M\<rbrakk> \<Longrightarrow> is_forcerel(##M,P,x,z) \<longleftrightarrow> z = forcerel(P,x)" 
-  unfolding is_forcerel_def forcerel_def 
+  "\<lbrakk>x\<in>M;z\<in>M\<rbrakk> \<Longrightarrow> is_forcerel(##M,P,x,z) \<longleftrightarrow> z = forcerel(P,x)"
+  unfolding is_forcerel_def forcerel_def
   using frecrel_abs names_below_abs trancl_abs P_in_M twoN_in_M ecloseN_closed names_below_closed
     names_below_productE[of concl:"\<lambda>p. is_frecrel(##M,p,_) \<longleftrightarrow>  _ = frecrel(p)"] frecrel_closed
   by simp
 
 lemma frc_at_abs:
-  assumes "fnnc\<in>M" "z\<in>M" 
+  assumes "fnnc\<in>M" "z\<in>M"
   shows "is_frc_at(##M,P,leq,fnnc,z) \<longleftrightarrow> z = frc_at(P,leq,fnnc)"
 proof -
   from assms
   have "(\<exists>r\<in>M. is_forcerel(##M,P,fnnc, r) \<and> is_wfrec(##M, is_Hfrc_at(##M, P, leq), r, fnnc, z))
         \<longleftrightarrow> is_wfrec(##M, is_Hfrc_at(##M, P, leq), forcerel(P,fnnc), fnnc, z)"
     using forcerel_abs forcerel_in_M by simp
-  then 
+  then
   show ?thesis
     unfolding frc_at_trancl is_frc_at_def
     using assms wfrec_Hfrc_at[of fnnc] wf_forcerel trans_forcerel_t relation_forcerel_t forcerel_in_M
@@ -1362,14 +1399,14 @@ lemma forces_mem'_abs :
 lemma forces_neq'_abs :
   assumes
     "p\<in>M" "t1\<in>M" "t2\<in>M"
-  shows 
+  shows
     "is_forces_neq'(##M,P,leq,p,t1,t2) \<longleftrightarrow> forces_neq'(P,leq,p,t1,t2)"
 proof -
   have "q\<in>M" if "q\<in>P" for q
     using that transitivity P_in_M by simp
   then show ?thesis
     unfolding is_forces_neq'_def forces_neq'_def
-    using assms forces_eq'_abs pair_in_M_iff 
+    using assms forces_eq'_abs pair_in_M_iff
     by (auto,blast)
 qed
 
@@ -1377,14 +1414,14 @@ qed
 lemma forces_nmem'_abs :
   assumes
     "p\<in>M" "t1\<in>M" "t2\<in>M"
-  shows 
+  shows
     "is_forces_nmem'(##M,P,leq,p,t1,t2) \<longleftrightarrow> forces_nmem'(P,leq,p,t1,t2)"
 proof -
   have "q\<in>M" if "q\<in>P" for q
     using that transitivity P_in_M by simp
   then show ?thesis
     unfolding is_forces_nmem'_def forces_nmem'_def
-    using assms forces_mem'_abs pair_in_M_iff 
+    using assms forces_mem'_abs pair_in_M_iff
     by (auto,blast)
 qed
 
@@ -1392,17 +1429,17 @@ end (* forcing_data *)
 
 subsection\<open>Forcing for general formulas\<close>
 
-definition 
+definition
   ren_forces_nand :: "i\<Rightarrow>i" where
   "ren_forces_nand(\<phi>) \<equiv> Exists(And(Equal(0,1),iterates(\<lambda>p. incr_bv(p)`1 , 2, \<phi>)))"
 
 lemma ren_forces_nand_type[TC] :
-  "\<phi>\<in>formula \<Longrightarrow> ren_forces_nand(\<phi>) \<in>formula" 
+  "\<phi>\<in>formula \<Longrightarrow> ren_forces_nand(\<phi>) \<in>formula"
   unfolding ren_forces_nand_def
   by simp
 
-lemma arity_ren_forces_nand : 
-  assumes "\<phi>\<in>formula" 
+lemma arity_ren_forces_nand :
+  assumes "\<phi>\<in>formula"
   shows "arity(ren_forces_nand(\<phi>)) \<le> succ(arity(\<phi>))"
 proof -
   consider (lt) "1<arity(\<phi>)" | (ge) "\<not> 1 < arity(\<phi>)"
@@ -1442,7 +1479,7 @@ proof -
 qed
 
 lemma sats_ren_forces_nand:
-  "[q,P,leq,o,p] @ env \<in> list(M) \<Longrightarrow> \<phi>\<in>formula \<Longrightarrow> 
+  "[q,P,leq,o,p] @ env \<in> list(M) \<Longrightarrow> \<phi>\<in>formula \<Longrightarrow>
    sats(M, ren_forces_nand(\<phi>),[q,p,P,leq,o] @ env) \<longleftrightarrow> sats(M, \<phi>,[q,P,leq,o] @ env)"
   unfolding ren_forces_nand_def
   using sats_incr_bv_iff [of _ _ M _ "[q]"]
@@ -1451,12 +1488,12 @@ lemma sats_ren_forces_nand:
 
 definition
   ren_forces_forall :: "i\<Rightarrow>i" where
-  "ren_forces_forall(\<phi>) \<equiv> 
+  "ren_forces_forall(\<phi>) \<equiv>
       Exists(Exists(Exists(Exists(Exists(
         And(Equal(0,6),And(Equal(1,7),And(Equal(2,8),And(Equal(3,9),
-        And(Equal(4,5),iterates(\<lambda>p. incr_bv(p)`5 , 5, \<phi>)))))))))))" 
+        And(Equal(4,5),iterates(\<lambda>p. incr_bv(p)`5 , 5, \<phi>)))))))))))"
 
-lemma arity_ren_forces_all : 
+lemma arity_ren_forces_all :
   assumes "\<phi>\<in>formula"
   shows "arity(ren_forces_forall(\<phi>)) = 5 \<union> arity(\<phi>)"
 proof -
@@ -1497,11 +1534,11 @@ proof -
 qed
 
 lemma ren_forces_forall_type[TC] :
-  "\<phi>\<in>formula \<Longrightarrow> ren_forces_forall(\<phi>) \<in>formula" 
+  "\<phi>\<in>formula \<Longrightarrow> ren_forces_forall(\<phi>) \<in>formula"
   unfolding ren_forces_forall_def by simp
 
 lemma sats_ren_forces_forall :
-  "[x,P,leq,o,p] @ env \<in> list(M) \<Longrightarrow> \<phi>\<in>formula \<Longrightarrow> 
+  "[x,P,leq,o,p] @ env \<in> list(M) \<Longrightarrow> \<phi>\<in>formula \<Longrightarrow>
     sats(M, ren_forces_forall(\<phi>),[x,p,P,leq,o] @ env) \<longleftrightarrow> sats(M, \<phi>,[p,P,leq,o,x] @ env)"
   unfolding ren_forces_forall_def
   using sats_incr_bv_iff [of _ _ M _ "[p,P,leq,o,x]"]
@@ -1510,16 +1547,16 @@ lemma sats_ren_forces_forall :
 
 definition
   is_leq :: "[i\<Rightarrow>o,i,i,i] \<Rightarrow> o" where
-  "is_leq(A,l,q,p) \<equiv> \<exists>qp[A]. (pair(A,q,p,qp) \<and> qp\<in>l)" 
+  "is_leq(A,l,q,p) \<equiv> \<exists>qp[A]. (pair(A,q,p,qp) \<and> qp\<in>l)"
 
 lemma (in forcing_data) leq_abs[simp]:
-  "\<lbrakk> l\<in>M ; q\<in>M ; p\<in>M \<rbrakk> \<Longrightarrow> is_leq(##M,l,q,p) \<longleftrightarrow> <q,p>\<in>l" 
+  "\<lbrakk> l\<in>M ; q\<in>M ; p\<in>M \<rbrakk> \<Longrightarrow> is_leq(##M,l,q,p) \<longleftrightarrow> <q,p>\<in>l"
   unfolding is_leq_def using pair_in_M_iff by simp
 
 
-definition 
+definition
   leq_fm :: "[i,i,i] \<Rightarrow> i" where
-  "leq_fm(leq,q,p) \<equiv> Exists(And(pair_fm(q#+1,p#+1,0),Member(0,leq#+1)))" 
+  "leq_fm(leq,q,p) \<equiv> Exists(And(pair_fm(q#+1,p#+1,0),Member(0,leq#+1)))"
 
 lemma arity_leq_fm :
   "\<lbrakk>leq\<in>nat;q\<in>nat;p\<in>nat\<rbrakk> \<Longrightarrow> arity(leq_fm(leq,q,p)) = succ(q) \<union> succ(p) \<union> succ(leq)"
@@ -1528,12 +1565,12 @@ lemma arity_leq_fm :
   by auto
 
 lemma leq_fm_type[TC] :
-  "\<lbrakk>leq\<in>nat;q\<in>nat;p\<in>nat\<rbrakk> \<Longrightarrow> leq_fm(leq,q,p)\<in>formula" 
+  "\<lbrakk>leq\<in>nat;q\<in>nat;p\<in>nat\<rbrakk> \<Longrightarrow> leq_fm(leq,q,p)\<in>formula"
   unfolding leq_fm_def by simp
 
 lemma sats_leq_fm :
-  "\<lbrakk> leq\<in>nat;q\<in>nat;p\<in>nat;env\<in>list(A) \<rbrakk> \<Longrightarrow> 
-     sats(A,leq_fm(leq,q,p),env) \<longleftrightarrow> is_leq(##A,nth(leq,env),nth(q,env),nth(p,env))" 
+  "\<lbrakk> leq\<in>nat;q\<in>nat;p\<in>nat;env\<in>list(A) \<rbrakk> \<Longrightarrow>
+     sats(A,leq_fm(leq,q,p),env) \<longleftrightarrow> is_leq(##A,nth(leq,env),nth(q,env),nth(p,env))"
   unfolding leq_fm_def is_leq_def by simp
 
 subsubsection\<open>The primitive recursion\<close>
@@ -1542,17 +1579,17 @@ consts forces' :: "i\<Rightarrow>i"
 primrec
   "forces'(Member(x,y)) = forces_mem_fm(1,2,0,x#+4,y#+4)"
   "forces'(Equal(x,y))  = forces_eq_fm(1,2,0,x#+4,y#+4)"
-  "forces'(Nand(p,q))   = 
+  "forces'(Nand(p,q))   =
         Neg(Exists(And(Member(0,2),And(leq_fm(3,0,1),And(ren_forces_nand(forces'(p)),
                                          ren_forces_nand(forces'(q)))))))"
-  "forces'(Forall(p))   = Forall(ren_forces_forall(forces'(p)))" 
+  "forces'(Forall(p))   = Forall(ren_forces_forall(forces'(p)))"
 
 
-definition 
+definition
   forces :: "i\<Rightarrow>i" where
   "forces(\<phi>) \<equiv> And(Member(0,1),forces'(\<phi>))"
 
-lemma forces'_type [TC]:  "\<phi>\<in>formula \<Longrightarrow> forces'(\<phi>) \<in> formula" 
+lemma forces'_type [TC]:  "\<phi>\<in>formula \<Longrightarrow> forces'(\<phi>) \<in> formula"
   by (induct \<phi> set:formula; simp)
 
 lemma forces_type[TC] : "\<phi>\<in>formula \<Longrightarrow> forces(\<phi>) \<in> formula"
@@ -1571,29 +1608,29 @@ definition
   forces_mem :: "[i,i,i] \<Rightarrow> o" where
   "forces_mem \<equiv> forces_mem'(P,leq)"
 
-(* frc_at(P,leq,<0,t1,t2,p>) = 1*) 
+(* frc_at(P,leq,<0,t1,t2,p>) = 1*)
 definition
   is_forces_eq :: "[i,i,i] \<Rightarrow> o" where
   "is_forces_eq \<equiv> is_forces_eq'(##M,P,leq)"
 
-(* frc_at(P,leq,<1,t1,t2,p>) = 1*) 
+(* frc_at(P,leq,<1,t1,t2,p>) = 1*)
 definition
   is_forces_mem :: "[i,i,i] \<Rightarrow> o" where
   "is_forces_mem \<equiv> is_forces_mem'(##M,P,leq)"
 
 
-lemma def_forces_eq: "p\<in>P \<Longrightarrow> forces_eq(p,t1,t2) \<longleftrightarrow> 
-      (\<forall>s\<in>domain(t1) \<union> domain(t2). \<forall>q. q\<in>P \<and> q \<preceq> p \<longrightarrow> 
-      (forces_mem(q,s,t1) \<longleftrightarrow> forces_mem(q,s,t2)))" 
-  unfolding forces_eq_def forces_mem_def forces_eq'_def forces_mem'_def 
-  using def_frc_at[of p 0 t1 t2 ]  unfolding bool_of_o_def 
+lemma def_forces_eq: "p\<in>P \<Longrightarrow> forces_eq(p,t1,t2) \<longleftrightarrow>
+      (\<forall>s\<in>domain(t1) \<union> domain(t2). \<forall>q. q\<in>P \<and> q \<preceq> p \<longrightarrow>
+      (forces_mem(q,s,t1) \<longleftrightarrow> forces_mem(q,s,t2)))"
+  unfolding forces_eq_def forces_mem_def forces_eq'_def forces_mem'_def
+  using def_frc_at[of p 0 t1 t2 ]  unfolding bool_of_o_def
   by auto
 
-lemma def_forces_mem: "p\<in>P \<Longrightarrow> forces_mem(p,t1,t2) \<longleftrightarrow> 
+lemma def_forces_mem: "p\<in>P \<Longrightarrow> forces_mem(p,t1,t2) \<longleftrightarrow>
      (\<forall>v\<in>P. v \<preceq> p \<longrightarrow>
       (\<exists>q. \<exists>s. \<exists>r. r\<in>P \<and> q\<in>P \<and> q \<preceq> v \<and> <s,r> \<in> t2 \<and> q \<preceq> r \<and> forces_eq(q,t1,s)))"
-  unfolding forces_eq'_def forces_mem'_def forces_eq_def forces_mem_def 
-  using def_frc_at[of p 1 t1 t2]  unfolding bool_of_o_def 
+  unfolding forces_eq'_def forces_mem'_def forces_eq_def forces_mem_def
+  using def_frc_at[of p 1 t1 t2]  unfolding bool_of_o_def
   by auto
 
 lemma forces_eq_abs :
@@ -1606,21 +1643,21 @@ lemma forces_mem_abs :
   unfolding is_forces_mem_def forces_mem_def
   using forces_mem'_abs by simp
 
-lemma sats_forces_eq_fm: 
-  assumes  "p\<in>nat" "l\<in>nat" "q\<in>nat" "t1\<in>nat" "t2\<in>nat"  "env\<in>list(M)" 
-    "nth(p,env)=P" "nth(l,env)=leq" 
-  shows "sats(M,forces_eq_fm(p,l,q,t1,t2),env) \<longleftrightarrow> 
+lemma sats_forces_eq_fm:
+  assumes  "p\<in>nat" "l\<in>nat" "q\<in>nat" "t1\<in>nat" "t2\<in>nat"  "env\<in>list(M)"
+    "nth(p,env)=P" "nth(l,env)=leq"
+  shows "sats(M,forces_eq_fm(p,l,q,t1,t2),env) \<longleftrightarrow>
          is_forces_eq(nth(q,env),nth(t1,env),nth(t2,env))"
-  unfolding forces_eq_fm_def is_forces_eq_def is_forces_eq'_def 
+  unfolding forces_eq_fm_def is_forces_eq_def is_forces_eq'_def
   using assms sats_is_tuple_fm  sats_frc_at_fm
   by simp
 
-lemma sats_forces_mem_fm: 
+lemma sats_forces_mem_fm:
   assumes  "p\<in>nat" "l\<in>nat" "q\<in>nat" "t1\<in>nat" "t2\<in>nat"  "env\<in>list(M)"
     "nth(p,env)=P" "nth(l,env)=leq"
-  shows "sats(M,forces_mem_fm(p,l,q,t1,t2),env) \<longleftrightarrow> 
+  shows "sats(M,forces_mem_fm(p,l,q,t1,t2),env) \<longleftrightarrow>
              is_forces_mem(nth(q,env),nth(t1,env),nth(t2,env))"
-  unfolding forces_mem_fm_def is_forces_mem_def is_forces_mem'_def 
+  unfolding forces_mem_fm_def is_forces_mem_def is_forces_mem'_def
   using assms sats_is_tuple_fm sats_frc_at_fm
   by simp
 
@@ -1635,53 +1672,53 @@ definition
 
 
 lemma forces_neq :
-  "forces_neq(p,t1,t2) \<longleftrightarrow> forces_neq'(P,leq,p,t1,t2)" 
+  "forces_neq(p,t1,t2) \<longleftrightarrow> forces_neq'(P,leq,p,t1,t2)"
   unfolding forces_neq_def forces_neq'_def forces_eq_def by simp
 
 lemma forces_nmem :
-  "forces_nmem(p,t1,t2) \<longleftrightarrow> forces_nmem'(P,leq,p,t1,t2)" 
+  "forces_nmem(p,t1,t2) \<longleftrightarrow> forces_nmem'(P,leq,p,t1,t2)"
   unfolding forces_nmem_def forces_nmem'_def forces_mem_def by simp
 
 
 lemma sats_forces_Member :
   assumes  "x\<in>nat" "y\<in>nat" "env\<in>list(M)"
-    "nth(x,env)=xx" "nth(y,env)=yy" "q\<in>M" 
-  shows "sats(M,forces(Member(x,y)),[q,P,leq,one]@env) \<longleftrightarrow> 
+    "nth(x,env)=xx" "nth(y,env)=yy" "q\<in>M"
+  shows "sats(M,forces(Member(x,y)),[q,P,leq,one]@env) \<longleftrightarrow>
                 (q\<in>P \<and> is_forces_mem(q,xx,yy))"
-  unfolding forces_def 
-  using assms sats_forces_mem_fm P_in_M leq_in_M one_in_M 
+  unfolding forces_def
+  using assms sats_forces_mem_fm P_in_M leq_in_M one_in_M
   by simp
 
 lemma sats_forces_Equal :
   assumes  "x\<in>nat" "y\<in>nat" "env\<in>list(M)"
-    "nth(x,env)=xx" "nth(y,env)=yy" "q\<in>M" 
-  shows "sats(M,forces(Equal(x,y)),[q,P,leq,one]@env) \<longleftrightarrow> 
+    "nth(x,env)=xx" "nth(y,env)=yy" "q\<in>M"
+  shows "sats(M,forces(Equal(x,y)),[q,P,leq,one]@env) \<longleftrightarrow>
                 (q\<in>P \<and> is_forces_eq(q,xx,yy))"
-  unfolding forces_def  
-  using assms sats_forces_eq_fm P_in_M leq_in_M one_in_M 
+  unfolding forces_def
+  using assms sats_forces_eq_fm P_in_M leq_in_M one_in_M
   by simp
 
 lemma sats_forces_Nand :
-  assumes  "\<phi>\<in>formula" "\<psi>\<in>formula" "env\<in>list(M)" "p\<in>M" 
-  shows "sats(M,forces(Nand(\<phi>,\<psi>)),[p,P,leq,one]@env) \<longleftrightarrow> 
-         (p\<in>P \<and> \<not>(\<exists>q\<in>M. q\<in>P \<and> is_leq(##M,leq,q,p) \<and> 
+  assumes  "\<phi>\<in>formula" "\<psi>\<in>formula" "env\<in>list(M)" "p\<in>M"
+  shows "sats(M,forces(Nand(\<phi>,\<psi>)),[p,P,leq,one]@env) \<longleftrightarrow>
+         (p\<in>P \<and> \<not>(\<exists>q\<in>M. q\<in>P \<and> is_leq(##M,leq,q,p) \<and>
                (sats(M,forces'(\<phi>),[q,P,leq,one]@env) \<and> sats(M,forces'(\<psi>),[q,P,leq,one]@env))))"
-  unfolding forces_def using sats_leq_fm assms sats_ren_forces_nand P_in_M leq_in_M one_in_M  
+  unfolding forces_def using sats_leq_fm assms sats_ren_forces_nand P_in_M leq_in_M one_in_M
   by simp
 
 lemma sats_forces_Neg :
-  assumes  "\<phi>\<in>formula" "env\<in>list(M)" "p\<in>M" 
-  shows "sats(M,forces(Neg(\<phi>)),[p,P,leq,one]@env) \<longleftrightarrow> 
-         (p\<in>P \<and> \<not>(\<exists>q\<in>M. q\<in>P \<and> is_leq(##M,leq,q,p) \<and> 
+  assumes  "\<phi>\<in>formula" "env\<in>list(M)" "p\<in>M"
+  shows "sats(M,forces(Neg(\<phi>)),[p,P,leq,one]@env) \<longleftrightarrow>
+         (p\<in>P \<and> \<not>(\<exists>q\<in>M. q\<in>P \<and> is_leq(##M,leq,q,p) \<and>
                (sats(M,forces'(\<phi>),[q,P,leq,one]@env))))"
   unfolding Neg_def using assms sats_forces_Nand
   by simp
 
 lemma sats_forces_Forall :
-  assumes  "\<phi>\<in>formula" "env\<in>list(M)" "p\<in>M" 
-  shows "sats(M,forces(Forall(\<phi>)),[p,P,leq,one]@env) \<longleftrightarrow> 
+  assumes  "\<phi>\<in>formula" "env\<in>list(M)" "p\<in>M"
+  shows "sats(M,forces(Forall(\<phi>)),[p,P,leq,one]@env) \<longleftrightarrow>
          p\<in>P \<and> (\<forall>x\<in>M. sats(M,forces'(\<phi>),[p,P,leq,one,x]@env))"
-  unfolding forces_def using assms sats_ren_forces_forall P_in_M leq_in_M one_in_M  
+  unfolding forces_def using assms sats_ren_forces_forall P_in_M leq_in_M one_in_M
   by simp
 
 end (* forcing_data *)
@@ -1693,7 +1730,7 @@ lemma arity_forces_at:
   shows "arity(forces(Member(x, y))) = (succ(x) \<union> succ(y)) #+ 4"
     "arity(forces(Equal(x, y))) = (succ(x) \<union> succ(y)) #+ 4"
   unfolding forces_def
-  using assms arity_forces_mem_fm arity_forces_eq_fm succ_Un_distrib nat_simp_union 
+  using assms arity_forces_mem_fm arity_forces_eq_fm succ_Un_distrib nat_simp_union
   by auto
 
 lemma arity_forces':
@@ -1727,7 +1764,7 @@ next
     from \<open>\<phi>\<in>_\<close> \<open>\<psi>\<in>_\<close>
     have A:"pred(arity(?\<phi>')) \<le> arity(forces'(\<phi>))"
       "pred(arity(?\<psi>')) \<le> arity(forces'(\<psi>))"
-      using pred_mono[OF _  arity_ren_forces_nand] pred_succ_eq 
+      using pred_mono[OF _  arity_ren_forces_nand] pred_succ_eq
       by simp_all
     from Nand
     have "3 \<union> arity(forces'(\<phi>)) \<le> arity(\<phi>) #+ 4"
@@ -1740,7 +1777,7 @@ next
       by simp_all
   qed
   with Nand \<open>_=4\<close>
-  show ?case 
+  show ?case
     using pred_Un_distrib Un_assoc[symmetric] succ_Un_distrib nat_union_abs1 Un_leI3[OF \<open>3 \<le> ?rhs\<close>]
     by simp
 next
@@ -1788,9 +1825,9 @@ next
   qed
 qed
 
-lemma arity_forces : 
+lemma arity_forces :
   assumes "\<phi>\<in>formula"
-  shows "arity(forces(\<phi>)) \<le> 4#+arity(\<phi>)" 
+  shows "arity(forces(\<phi>)) \<le> 4#+arity(\<phi>)"
   unfolding forces_def
   using assms arity_forces' le_trans nat_simp_union by auto
 
